evolution!!!!

LCNova.v
@@ -1,1430 +1,2285 @@
-From Coq.Bool Require Export Bool.
-From Coq.micromega Require Export Lia.
-From Coq.Lists Require Export List.
-From Coq.Arith Require Export PeanoNat.
-From Coq.Program Require Export Equality.
+Require Import Coq.Bool.Bool.
+Require Import Coq.Arith.PeanoNat.
+Require Import Coq.Lists.List.
+Require Import Coq.micromega.Lia.
+Require Import Coq.Classes.RelationClasses.
+Require Import Coq.Logic.Classical.
 
-Module AuxiliaPalatina.  
+Module AuxiliaryPalatina.
 
-  Import ListNotations.
+Import ListNotations.
 
-  Section forNat.
+Section Utilities.
 
-  Theorem SecondPrincipleOfFiniteInduction (phi : nat -> Prop) :
-    let phi' : nat -> Prop := fun k : nat => (forall i : nat, i < k -> phi i) in
-    (forall k : nat, phi' k -> phi k) ->
-    (forall n : nat, phi n).
-  Proof.
-    intros phi'.
-    intro.
-    cut (
-      (forall n : nat, phi n /\ phi' n)
-    ).
-      intro.
-      intros n.
-      destruct (H0 n).
-      apply H1.
-    intros n.
-    induction n.
-    - assert (phi' 0).
-        intros i.
-        lia.
-      constructor.
-      apply H.
-      apply H0.
-      apply H0.
-    - assert (phi' (S n)).
-        intros i.
-        intro.
-        inversion H0.
-        destruct IHn.
-        apply H1.
-        subst.
-        destruct IHn.
-        apply (H3 i).
-        lia.
-      constructor.
-      apply H.
-      apply H0.
-      apply H0.
-  Qed.
+Definition case_eq {A : Type} : forall x : A, forall y : A, forall phi : forall x0 : A, x0 = y -> Type, phi y eq_refl -> forall H : x = y, phi x H :=
+  fun x : A =>
+  fun y : A =>
+  fun phi : forall x0 : A, x0 = y -> Type =>
+  fun phi_y : phi y eq_refl =>
+  fun H : eq x y =>
+  match H as H0 in eq _ y0 return forall phi0 : forall x0 : A, x0 = y0 -> Type, phi0 y0 eq_refl -> phi0 x H0 with
+  | eq_refl =>
+    fun phi0 : forall x0 : A, x0 = x -> Type =>
+    fun phi_y0 : phi0 x eq_refl =>
+    phi_y0
+  end phi phi_y
+.
 
-  Fixpoint first_nat (p : nat -> bool) (n : nat) : nat :=
-    match n with
-    | 0 => 0
-    | S n' =>
-      if p (first_nat p n')
-      then first_nat p n'
-      else n
+Lemma div_mod_uniqueness :
+  forall a : nat,
+  forall b : nat,
+  forall q : nat,
+  forall r : nat,
+  a = b * q + r ->
+  r < b ->
+  a / b = q /\ a mod b = r.
+Proof with try (lia || now (firstorder; eauto)).
+  assert (H : forall x : nat, forall y : nat, x > y <-> (exists z : nat, x = S (y + z))).
+  { intros x y; constructor.
+    - intros H.
+      induction H...
+      destruct IHle as [z H0].
+      exists (S z)...
+    - intros H.
+      destruct H as [z H]...
+  }
+  intros a b q r H1 H2.
+  assert (H0 : a = b * (a / b) + (a mod b)) by now apply (Nat.div_mod a b); lia.
+  assert (H3 : 0 <= a mod b < b) by now apply (Nat.mod_bound_pos a b); lia.
+  assert (H4 : ~ q > a / b).
+  { intros H4.
+    enough (H5 : exists z : nat, q = S (a / b + z))...
+    destruct H5 as [z H5].
+    enough (b * q + r >= b * S (a / b) + r)...
+  }
+  assert (H5 : ~ q < a / b).
+  { intros H5.
+    enough (H6 : exists z : nat, a / b = S (q + z))...
+    destruct H6 as [z H6].
+    enough (b * q + a mod b >= b * S (a / b) + a mod b)...
+  }
+  enough (q = a / b)...
+Qed.
+
+Definition first_nat : (nat -> bool) -> nat -> nat :=
+  fun p : nat -> bool =>
+  fix first_nat_fix (n : nat) {struct n} : nat :=
+  match n with
+  | 0 => 0
+  | S n' => if p (first_nat_fix n') then first_nat_fix n' else n
+  end
+.
+
+Theorem well_ordering_principle : 
+  forall p : nat -> bool,
+  forall n : nat,
+  p n = true ->
+  let m : nat := first_nat p n in
+  p m = true /\ (forall i : nat, p i = true -> i >= m).
+Proof with eauto. (* This proof has been improved by JunYoung Clare Jang. *)
+  intros p n H3 m.
+  assert (forall x : nat, p x = true -> p (first_nat p x) = true).
+  { induction x...
+    simpl.
+    destruct (p (first_nat p x)) eqn:H0...
+  }
+  split...
+  intros i H4.
+  enough (forall x : nat, first_nat p x <= x).
+  enough (forall x : nat, p (first_nat p x) = true -> (forall y : nat, x < y -> first_nat p x = first_nat p y)).
+  enough (forall x : nat, forall y : nat, p y = true -> first_nat p x <= y)...
+  - intros x y H2.
+    destruct (Compare_dec.le_lt_dec x y).
+    + eapply Nat.le_trans...
+    + replace (first_nat p x) with (first_nat p y)...
+  - intros x H1 y H2.
+    induction H2; simpl.
+    + rewrite H1...
+    + rewrite <- IHle, H1...
+  - induction x...
+    simpl.
+    destruct (p (first_nat p x)) eqn: H0...
+Qed.
+
+Fixpoint sum_from_0_to (n : nat) {struct n} : nat :=
+  match n with
+  | 0 => 0
+  | S n' => n + sum_from_0_to n'
+  end
+.
+
+Proposition sum_from_0_to_is :
+  forall n : nat,
+  2 * sum_from_0_to n = n * (S n).
+Proof with lia.
+  induction n; simpl in *...
+Qed.
+
+Fixpoint cantor_pairing (n : nat) {struct n} : nat * nat :=
+  match n with
+  | 0 => (0, 0)
+  | S n' =>
+    match cantor_pairing n' with
+    | (0, y) => (S y, 0)
+    | (S x, y) => (x, S y)
     end
-  .
+  end
+.
 
-  Lemma well_ordering_principle : 
-    forall p : nat -> bool,
-    forall n : nat,
-    p n = true ->
-    let m : nat := first_nat p n in
-    p m = true /\ (forall i : nat, p i = true -> i >= m).
-  Proof.
-    intros p.
-    assert (forall x : nat, p x = true -> p (first_nat p x) = true).
-      intros x.
-      induction x.
-      tauto.
+Lemma cantor_pairing_is_surjective :
+  forall x : nat,
+  forall y : nat,
+  (x, y) = cantor_pairing (sum_from_0_to (x + y) + y).
+Proof with (lia || eauto).
+  enough (forall z : nat, forall y : nat, forall x : nat, z = x + y -> (x, y) = cantor_pairing (sum_from_0_to z + y))...
+  induction z.
+  - intros y x H.
+    assert (H0 : x = 0)...
+    assert (H1 : y = 0)...
+    subst...
+  - induction y.
+    + intros x H.
+      assert (H0 : x = S z)...
+      subst.
       simpl.
-      cut (let b : bool := p (first_nat p x) in p (S x) = true -> p (if b then first_nat p x else S x) = true).
+      destruct (cantor_pairing (z + sum_from_0_to z + 0)) eqn: H0.
+      assert (H1 : (0, z) = cantor_pairing (sum_from_0_to z + z))...
+      rewrite Nat.add_0_r, Nat.add_comm in H0.
+      rewrite H0 in H1.
+      inversion H1; subst...
+    + intros x H.
+      enough (H0 : (S x, y) = cantor_pairing (sum_from_0_to (S z) + y)).
+      { assert (H1 : z + sum_from_0_to z + S y = sum_from_0_to (S z) + y) by now simpl...
         simpl.
-        tauto.
+        rewrite H1, <- H0...
+      }
+      apply (IHy (S x))...
+Qed.
+
+Lemma cantor_pairing_is_injective :
+  forall n : nat,
+  forall x : nat,
+  forall y : nat,
+  cantor_pairing n = (x, y) ->
+  n = sum_from_0_to (x + y) + y.
+Proof with (lia || eauto).
+  induction n; simpl.
+  - intros x y H.
+    inversion H; subst...
+  - intros x y H.
+    destruct (cantor_pairing n) as [x' y'] eqn: H0.
+    destruct x'; (inversion H; subst).
+    + repeat (rewrite Nat.add_0_r).
+      simpl.
+      rewrite (IHn 0 y' eq_refl), Nat.add_0_l...
+    + rewrite (IHn (S x) y' eq_refl).
+      assert (H1 : forall x' : nat, S x' + y' = x' + S y')...
+      repeat (rewrite H1)...
+Qed.
+
+Corollary cantor_pairing_is :
+  forall n : nat,
+  forall x : nat,
+  forall y : nat,
+  cantor_pairing n = (x, y) <-> n = sum_from_0_to (x + y) + y.
+Proof with eauto using cantor_pairing_is_injective, cantor_pairing_is_surjective.
+  split...
+  intros H.
+  subst...
+Qed.
+
+Definition S_0 {A : Type} : forall n : nat, S n = 0 -> A :=
+  fun n : nat =>
+  fun H0 : S n = 0 =>
+  let H1 : 0 = S n := @eq_ind nat (S n) (fun x : nat => x = S n) eq_refl 0 H0 in
+  let H2 : False := @eq_ind nat 0 (fun x : nat => if Nat.eqb x 0 then True else False) I (S n) H1 in
+  False_rect A H2
+.
+
+Definition S_S : forall n1 : nat, forall n2 : nat, S n1 = S n2 -> n1 = n2 :=
+  fun n1 : nat =>
+  fun n2 : nat =>
+  fun H0 : S n1 = S n2 =>
+  @eq_ind nat (S n1) (fun x : nat => n1 = pred x) eq_refl (S n2) H0
+.
+
+Inductive FinSet : nat -> Set :=
+| FZ : forall n : nat, FinSet (S n) 
+| FS : forall n : nat, FinSet n -> FinSet (S n)
+.
+
+Definition FinSet_case0 {P : FinSet 0 -> Type} : forall i : FinSet 0, P i :=
+  fun i : FinSet 0 =>
+  match i as i0 in FinSet Sn return Sn = 0 -> P i with
+  | FZ n => S_0 n
+  | FS n i' => S_0 n
+  end eq_refl
+.
+
+Definition FinSet_caseS {n : nat} {P : FinSet (S n) -> Type} : P (FZ n) -> (forall i' : FinSet n, P (FS n i')) -> (forall i : FinSet (S n), P i) :=
+  fun PZ : P (FZ n) =>
+  fun PS : forall i' : FinSet n, P (FS n i') =>
+  fun i : FinSet (S n) =>
+  match i as i0 in FinSet Sn0 return (match Sn0 as Sn1 return FinSet Sn1 -> Type with 0 => FinSet_case0 | S n0 => fun i1 : FinSet (S n0) => forall P0 : FinSet (S n0) -> Type, P0 (FZ n0) -> (forall i' : FinSet n0, P0 (FS n0 i')) -> P0 i1 end) i0 with
+  | FZ n0 => fun P0 : FinSet (S n0) -> Type => fun PZ0 : P0 (FZ n0) => fun PS0 : forall i' : FinSet n0, P0 (FS n0 i') => PZ0
+  | FS n0 i' => fun P0 : FinSet (S n0) -> Type => fun PZ0 : P0 (FZ n0) => fun PS0 : forall i' : FinSet n0, P0 (FS n0 i') => PS0 i'
+  end P PZ PS
+.
+
+Definition FinSet_rectS {P : forall n : nat, FinSet n -> Type} : (forall n : nat, P (S n) (FZ n)) -> (forall n : nat, forall i' : FinSet n, P n i' -> P (S n) (FS n i')) -> (forall n : nat, forall i : FinSet (S n), P (S n) i) :=
+  fun PZ : forall n : nat, P (S n) (FZ n) =>
+  fun PS : forall n : nat, forall i' : FinSet n, P n i' -> P (S n) (FS n i') =>
+  fix FinSet_rectS_fix (n : nat) (i : FinSet (S n)) {struct i} : P (S n) i :=
+  match i as i0 in FinSet Sn0 return P Sn0 i0 with
+  | FZ n0 => PZ n0
+  | FS n0 i' =>
+    match n0 as n1 return forall i0' : FinSet n1, P (S n1) (FS n1 i0') with
+    | 0 => fun i0' : FinSet 0 => @FinSet_case0 (fun i1 : FinSet 0 => P 1 (FS 0 i1)) i0'
+    | S n0' => fun i0' : FinSet (S n0') => PS (S n0') i0' (FinSet_rectS_fix n0' i0')
+    end i'
+  end
+.
+
+Lemma forallb_true_iff {A : Type} {p : A -> bool} (xs : list A) :
+  forallb p xs = true <-> forall x : A, In x xs -> p x = true.
+Proof with try now firstorder.
+  induction xs; simpl...
+  rewrite andb_true_iff.
+  split...
+  intros H0 x H1.
+  destruct H0; destruct H1...
+  rewrite H1 in H...
+Qed.
+
+Definition fold_right_max_0 : list nat -> nat :=
+  fold_right max 0
+.
+
+Lemma fold_right_max_0_in :
+  forall ns : list nat,
+  forall n : nat,
+  In n ns ->
+  fold_right_max_0 ns >= n.
+Proof with (lia || eauto).
+  unfold fold_right_max_0.
+  induction ns as [| n' ns]; simpl...
+  intros n H.
+  destruct H...
+  enough (fold_right max 0 ns >= n)...
+Qed.
+
+Lemma fold_right_max_0_app :
+  forall ns1 : list nat,
+  forall ns2 : list nat,
+  fold_right_max_0 (ns1 ++ ns2) = max (fold_right_max_0 ns1) (fold_right_max_0 ns2).
+Proof with (lia || eauto).
+  unfold fold_right_max_0.
+  induction ns1 as [| n1 ns1]; simpl... 
+  intros n.
+  rewrite IHns1...
+Qed.
+
+Lemma property1_of_fold_right_max_0 (Phi : nat -> Prop) (Phi_dec : forall i : nat, {Phi i} + {~ Phi i}) :
+  forall ns : list nat,
+  (forall i : nat, Phi i -> In i ns) ->
+  forall n : nat,
+  Phi n ->
+  fold_right max 0 ns >= n.
+Proof with (lia || eauto).
+  induction ns; simpl.
+  - intros H n H0.
+    contradiction (H n).
+  - intros H n H0.
+    destruct (Compare_dec.le_lt_dec n a)...
+    enough (fold_right max 0 ns >= n)...
+    destruct (Phi_dec n).
+    + destruct (H n p)...
+      enough (forall ks : list nat, forall k : nat, In k ks -> fold_right max 0 ks >= k) by firstorder.
+      induction ks; simpl...
+      intros k H2.
+      destruct H2...
+      enough (fold_right Init.Nat.max 0 ks >= k)...
+    + apply IHns...
       intros.
-      assert (b = true \/ b = false).
-        destruct b.
-          tauto.
-          tauto.
-      destruct H0.
-      rewrite H0.
-      unfold b in H0.
-      apply H0.
-      rewrite H0.
-      apply H.
-    assert (forall x : nat, first_nat p x <= x).
-      intros x.
-      induction x.
-        simpl.
-        lia.
-        simpl.
-        cut (let b : bool := p (first_nat p x) in (if b then first_nat p x else S x) <= S x).
-          simpl.
-          tauto.
-        intros.
-        assert (b = true \/ b = false).
-          destruct b.
-            tauto.
-            tauto.
-        destruct H0.
-          rewrite H0.
-          lia.
-          rewrite H0.
-          lia.
-    assert (forall x : nat, p (first_nat p x) = true -> (forall y : nat, x < y -> first_nat p x = first_nat p y)).
-      intros x.
-      intro.
-      intros y.
-      intro.
-      induction H2.
-        simpl.
-        rewrite H1.
-        tauto.
-        simpl.
-        rewrite <- IHle.
-        rewrite H1.
-        tauto.
-    assert (forall x : nat, forall y : nat, p y = true -> first_nat p x <= y).
-      intros x.
-      intros y.
-      intro.
-      assert (x <= y \/ x > y).
-        lia.
-      destruct H3.
-      assert (first_nat p x <= x <= y).
-        constructor.
-        apply (H0 x).
-        apply H3.
-        lia.
-      assert (p (first_nat p y) = true).
-        apply (H y).
-        assert (first_nat p x <= x).
-          apply (H0 x).
-          apply H2.
-      assert (first_nat p y = first_nat p x).
-        apply (H1 y).
-        apply H4.
-        lia.
-        rewrite <- H5.
-        apply (H0 y).
-    intros n.
-    intro.
-    intros m.
-    constructor.
-    unfold m.
-    apply (H n H3).
-    intros i.
-    intro.
-    assert (first_nat p n <= i).
-      apply (H2 n i H4).
-    unfold m.
-    apply H5.
-  Qed.
+      destruct (H i H1)...
+      subst.
+      contradiction.
+Qed.
 
-  Theorem WellOrderingPrinciple :
-    forall Phi : nat -> Prop,
-    (forall i : nat, {Phi i} + {~ Phi i}) ->
-    {n : nat | Phi n} ->
-    {m : nat | Phi m /\ (forall i : nat, Phi i -> i >= m)}.
-  Proof.
-    intros Phi H_Phi_dec H_n_exists.
-    destruct H_n_exists as [n].
-    destruct (well_ordering_principle (fun i : nat => if H_Phi_dec i then true else false) n).
-    destruct (H_Phi_dec n).
-    tauto.
-    tauto.
-    exists (first_nat (fun i : nat => if H_Phi_dec i then true else false) n).
-    constructor.
-    destruct (H_Phi_dec (first_nat (fun i : nat => if H_Phi_dec i then true else false) n)).
-    apply p0.
-    contradiction n0.
-    inversion H.
-    intros i.
-    intro.
-    apply H0.
-    destruct (H_Phi_dec i).
-    tauto.
-    tauto.
-  Qed.
+Lemma property2_of_fold_right_max_0 :
+  forall ns : list nat,
+  forall n : nat,
+  fold_right max 0 ns > n <-> (exists i : nat, In i ns /\ i > n).
+Proof with (lia || eauto).
+  induction ns; simpl.
+  - split...
+    now firstorder.
+  - intros n.
+    destruct (Compare_dec.le_lt_dec a (fold_right Init.Nat.max 0 ns)); split...
+    + intros H.
+      assert (H0 : fold_right Init.Nat.max 0 ns > n)...
+      destruct (proj1 (IHns n) H0) as [i].
+      now firstorder.
+    + intros H.
+      destruct H as [i].
+      destruct H.
+      destruct H.
+      * subst...
+      * enough (fold_right max 0 ns > n)...
+        apply IHns...
+    + intros H.
+      exists a...
+    + intros H.
+      destruct H as [i].
+      destruct H.
+      destruct H.
+      * subst...
+      * enough (fold_right Init.Nat.max 0 ns > n)...
+        apply IHns...
+Qed.
 
-  End forNat.
+Lemma property3_of_fold_right_max_0 :
+  forall ns1 : list nat,
+  forall ns2 : list nat,
+  fold_right max 0 (ns1 ++ ns2) = max (fold_right max 0 ns1) (fold_right max 0 ns2).
+Proof.
+  apply fold_right_max_0_app.
+Qed.
 
-  Section forFinSet.
+Lemma property4_of_fold_right_max_0 :
+  forall ns : list nat,
+  forall n : nat,
+  In n ns ->
+  fold_right max 0 ns >= n.
+Proof with (lia || eauto).
+  induction ns; simpl...
+  intros n H.
+  destruct H...
+  enough (fold_right max 0 ns >= n)...
+Qed.
 
-  Inductive FinSet : nat -> Set :=
-  | FinSetZ :
-    forall n : nat,
-    FinSet (S n)
-  | FinSetS :
-    forall n : nat,
-    FinSet n ->
-    FinSet (S n)
-  .
+Lemma property5_of_fold_right_max_0 :
+  forall ns1 : list nat,
+  forall ns2 : list nat,
+  (forall n : nat, In n ns1 -> In n ns2) ->
+  fold_right max 0 ns1 <= fold_right max 0 ns2.
+Proof with (lia || eauto).
+  induction ns1; simpl...
+  intros ns2 H.
+  destruct (Compare_dec.le_lt_dec a (fold_right max 0 ns1)).
+  - enough (fold_right max 0 ns1 <= fold_right max 0 ns2)...
+  - enough (a <= fold_right max 0 ns2)...
+    apply property4_of_fold_right_max_0...
+Qed.
 
-  Lemma makeFinSet :
-    forall n : nat,
-    forall i : nat,
-    i < n ->
-    FinSet n.
-  Proof.
-    intros n.
-    induction n.
-    - intros.
-      lia.
-    - intros.
-      destruct (Nat.eq_dec i n).
-      * apply FinSetZ.
-      * apply FinSetS.
-        apply (IHn i).
-        lia.
-  Qed.
+Lemma fold_right_max_0_ext :
+  forall ns1 : list nat,
+  forall ns2 : list nat,
+  (forall n : nat, In n ns1 <-> In n ns2) ->
+  fold_right max 0 ns1 = fold_right max 0 ns2.
+Proof with try now firstorder.
+  intros.
+  enough (fold_right max 0 ns1 <= fold_right max 0 ns2 /\ fold_right max 0 ns2 <= fold_right max 0 ns1) by lia.
+  split; apply property5_of_fold_right_max_0...
+Qed.
 
-  Lemma runFinSet :
-    forall n : nat,
-    FinSet n ->
-    {i : nat | i < n}.
-  Proof.
+End Utilities.
+
+#[global] Create HintDb naive_set_theory.
+
+Definition Ensemble (A : Type) : Type :=
+  A -> Prop
+.
+
+Definition member {A : Type} : A -> Ensemble A -> Prop :=
+  fun x : A => fun xs : Ensemble A => xs x
+.
+
+#[global] Hint Unfold member : naive_set_theory.
+
+Definition isSubsetOf {A : Type} : Ensemble A -> Ensemble A -> Prop :=
+  fun xs1 : Ensemble A => fun xs2 : Ensemble A => forall x : A, member x xs1 -> member x xs2
+.
+
+#[global] Hint Unfold isSubsetOf : naive_set_theory.
+
+Inductive full {A : Type} : Ensemble A :=
+| In_full {x : A} : member x full
+.
+
+#[global] Hint Constructors full : naive_set_theory.
+
+Inductive empty {A : Type} : Ensemble A :=
+.
+
+#[global] Hint Constructors empty : naive_set_theory.
+
+Inductive singleton {A : Type} : A -> Ensemble A :=
+| In_singleton {x : A} : member x (singleton x)
+.
+
+#[global] Hint Constructors singleton : naive_set_theory.
+
+Inductive unions {A : Type} : Ensemble (Ensemble A) -> Ensemble A :=
+| In_unions {x : A} {xss : Ensemble (Ensemble A)} : forall xs : Ensemble A, member x xs -> member xs xss -> member x (unions xss)
+.
+
+#[global] Hint Constructors unions : naive_set_theory.
+
+Inductive union {A : Type} : Ensemble A -> Ensemble A -> Ensemble A :=
+| Inl_union {x : A} {xs1 : Ensemble A} {xs2 : Ensemble A} : member x xs1 -> member x (union xs1 xs2)
+| Inr_union {x : A} {xs1 : Ensemble A} {xs2 : Ensemble A} : member x xs2 -> member x (union xs1 xs2)
+.
+
+#[global] Hint Constructors union : naive_set_theory.
+
+Inductive intersection {A : Type} : Ensemble A -> Ensemble A -> Ensemble A :=
+| In_intersection {x : A} {xs1 : Ensemble A} {xs2 : Ensemble A} : member x xs1 -> member x xs2 -> member x (intersection xs1 xs2)
+.
+
+#[global] Hint Constructors intersection : naive_set_theory.
+
+Inductive image {A : Type} {B : Type} : (A -> B) -> Ensemble A -> Ensemble B :=
+| In_image {xs : Ensemble A} : forall x : A, forall f : A -> B, member x xs -> member (f x) (image f xs)
+.
+
+#[global] Hint Constructors image : naive_set_theory.
+
+Inductive inverse_image {A : Type} {B : Type} : (A -> B) -> Ensemble B -> Ensemble A :=
+| In_inverse_image {f : A -> B} {ys : Ensemble B} : forall x : A, member (f x) ys -> member x (inverse_image f ys)
+.
+
+#[global] Hint Constructors inverse_image : naive_set_theory.
+
+Definition NonEmpty {A : Type} : Ensemble A -> Prop :=
+  fun xs : Ensemble A => exists x : A, member x xs
+.
+
+#[global] Hint Unfold NonEmpty : naive_set_theory.
+
+End AuxiliaryPalatina.
+
+Module DomainTheory.
+
+Import ListNotations.
+
+Import AuxiliaryPalatina.
+
+#[global] Create HintDb domain_theory_hints.
+
+Class TopologicalSpace (X : Set) : Type :=
+  { is_open_set : Ensemble X -> Prop
+  ; open_set_for_full :
+    is_open_set full
+  ; open_set_for_unions :
+    forall xss : Ensemble (Ensemble X),
+    (forall xs : Ensemble X, member xs xss -> is_open_set xs) ->
+    is_open_set (unions xss)
+  ; open_set_for_intersection :
+    forall xs1 : Ensemble X,
+    forall xs2 : Ensemble X,
+    is_open_set xs1 ->
+    is_open_set xs2 ->
+    is_open_set (intersection xs1 xs2)
+  }
+.
+
+#[global] Hint Resolve open_set_for_full : domain_theory_hints.
+
+#[global] Hint Resolve open_set_for_unions : domain_theory_hints.
+
+#[global] Hint Resolve open_set_for_intersection : domain_theory_hints.
+
+Definition is_continuous_map {X : Set} {Y : Set} `{X_is_topology : TopologicalSpace X} `{Y_is_topology : TopologicalSpace Y} : (X -> Y) -> Prop :=
+  fun f : X -> Y => forall ys : Ensemble Y, is_open_set ys -> is_open_set (inverse_image f ys)
+.
+
+#[global] Hint Unfold is_continuous_map : domain_theory_hints.
+
+Class Poset_minor (X : Set) : Type :=
+  { eql : X -> X -> Prop
+  ; leq : X -> X -> Prop
+  ; requriesEquivalence :> Equivalence eql
+  ; requiresPreOrder :> PreOrder leq
+  ; requiresPartialOrder :> PartialOrder eql leq
+  }
+.
+
+Local Notation "x =-= y" := (eql x y) (at level 70, no associativity) : type_scope.
+
+Class Poset (Y : Set) : Type :=
+  { requiresPoset_minor :> Poset_minor Y
+  ; substitutablity {X : Set} {requiresPoset_minor : Poset_minor X} : forall x1 : X, forall x2 : X, x1 =-= x2 -> forall f : X -> Y, f x1 =-= f x2
+  }
+.
+
+#[global] Hint Resolve substitutablity : domain_theory_hints.
+
+Lemma leq_refl1 {D : Set} `{D_is_poset_minor : Poset_minor D} :
+  forall x1 : D,
+  forall x2 : D,
+  x1 =-= x2 ->
+  leq x1 x2.
+Proof with eauto.
+  intros.
+  apply partial_order_equivalence in H.
+  destruct H...
+Qed.
+
+#[global] Hint Resolve leq_refl1 : domain_theory_hints.
+
+Lemma leq_refl2 {D : Set} `{D_is_poset_minor : Poset D} :
+  forall x1 : D,
+  forall x2 : D,
+  x1 =-= x2 ->
+  leq x2 x1.
+Proof with eauto.
+  intros.
+  apply partial_order_equivalence in H.
+  destruct H...
+Qed.
+
+#[global] Hint Resolve leq_refl2 : domain_theory_hints.
+
+Lemma leq_asym {D : Set} `{D_is_poset_minor : Poset_minor D} :
+  forall x1 : D,
+  forall x2 : D,
+  leq x1 x2 ->
+  leq x2 x1 ->
+  x1 =-= x2.
+Proof with eauto.
+  intros.
+  apply antisymmetry...
+Qed.
+
+#[global] Hint Resolve leq_asym : domain_theory_hints.
+
+Lemma leq_trans {D : Set} `{D_is_poset_minor : Poset_minor D} :
+  forall x1 : D,
+  forall x2 : D,
+  forall x3 : D,
+  leq x1 x2 ->
+  leq x2 x3 ->
+  leq x1 x3.
+Proof.
+  intros.
+  apply (transitivity (R:=leq) H H0).
+Qed.
+
+#[global] Hint Resolve leq_trans : domain_theory_hints.
+
+Definition directed {D : Set} `{D_is_poset : Poset D} : Ensemble D -> Prop :=
+  fun X : Ensemble D => NonEmpty X /\ (forall x1 : D, member x1 X -> forall x2 : D, member x2 X -> exists x3 : D, member x3 X /\ leq x1 x3 /\ leq x2 x3)
+.
+
+#[global] Hint Unfold directed : domain_theory_hints.
+
+Definition is_supremum {D : Set} `{D_is_poset : Poset D} : D -> Ensemble D -> Prop :=
+  fun sup_xs : D => fun xs : Ensemble D => forall x : D, leq sup_xs x <-> (forall x0 : D, member x0 xs -> leq x0 x)
+.
+
+#[global] Hint Unfold is_supremum : domain_theory_hints.
+
+Lemma supremum_unique {D : Set} `{D_is_poset_minor : Poset D} :
+  forall X : Ensemble D,
+  forall x1 : D,
+  forall x2 : D,
+  is_supremum x1 X ->
+  is_supremum x2 X <-> x1 =-= x2.
+Proof with eauto with *.
+  intros X x1 x2 H1.
+  split; intros H2.
+  - apply leq_asym.
+    + apply H1.
+      intros x H.
+      apply H2...
+    + apply H2.
+      intros x H.
+      apply H1...
+  - intros x.
+    split.
+    + intros H3 x' H4.
+      apply H1...
+    + intros H4.
+      apply (leq_trans x2 x1 x)...
+      apply H1...
+Qed.
+
+#[global] Hint Resolve supremum_unique : domain_theory_hints.
+
+Lemma supremum_ext {D : Set} `{D_is_poset_minor : Poset D} :
+  forall X1 : Ensemble D,
+  forall X2 : Ensemble D,
+  isSubsetOf X1 X2 ->
+  isSubsetOf X2 X1 ->
+  forall x1 : D,
+  forall x2 : D,
+  is_supremum x1 X1 ->
+  is_supremum x2 X2 <-> x1 =-= x2.
+Proof with eauto with *.
+  intros X1 X2 H H0 x1 x2 H1.
+  split; intros H2.
+  - apply leq_asym.
+    + apply H1.
+      intros x H3.
+      apply H2...
+    + apply H2.
+      intros x H3.
+      apply H1...
+  - intros x.
+    split.
+    + intros H3 x' H4.
+      apply H1...
+    + intros H4.
+      apply (leq_trans x2 x1 x)...
+      apply H1...
+Qed.
+
+#[global] Hint Resolve supremum_ext : domain_theory_hints.
+
+Class CompletePartialOrder (D : Set) `{requiresPoset : Poset D} : Type :=
+  { bottom : D
+  ; bottom_least :
+    forall x : D,
+    leq bottom x
+  ; supremum_exists :
+    forall xs : Ensemble D,
+    directed xs ->
+    {sup_xs : D | is_supremum sup_xs xs}
+  }
+.
+
+#[global] Hint Resolve bottom_least : domain_theory_hints.
+
+#[global] Hint Resolve supremum_exists : domain_theory_hints.
+
+Class CompleteLattice (D : Set) `{requiresPoset : Poset D} : Type :=
+  { supremum_always_exists :
+    forall xs : Ensemble D,
+    {sup_xs : D | is_supremum sup_xs xs}
+  }
+.
+
+#[global] Hint Resolve supremum_always_exists : domain_theory_hints.
+
+Global Program Instance each_complete_lattice_is_a_cpo (D : Set) `{D_is_poset : Poset D} (requiresCompleteLattice : CompleteLattice D) : CompletePartialOrder D :=
+  { bottom := supremum_always_exists empty
+  }
+.
+
+Next Obligation with eauto with naive_set_theory.
+  assert (H := proj2_sig (supremum_always_exists empty)).
+  simpl in H.
+  apply H.
+  intros.
+  inversion H0.
+Qed.
+
+Next Obligation with eauto with naive_set_theory.
+  apply supremum_always_exists.
+Qed.
+
+Global Program Instance scott_topology (D : Set) `{D_is_poset : Poset D} (requiresCompletePartialOrder : CompletePartialOrder D) : TopologicalSpace D :=
+  { is_open_set := fun O : Ensemble D => (forall x : D, forall y : D, member x O -> leq x y -> member y O) /\ (forall X : Ensemble D, directed X -> forall sup_X : D, is_supremum sup_X X -> member sup_X O -> NonEmpty (intersection X O))
+  }
+.
+
+Next Obligation with eauto with *.
+  split...
+  intros.
+  destruct H.
+  destruct H.
+  exists x...
+Qed.
+
+Next Obligation with eauto with *.
+  split.
+  - intros.
+    destruct H0.
+    apply (In_unions xs)...
+    apply (proj1 (H xs H2) x y)...
+  - intros.
+    inversion H0; subst.
+    inversion H2; subst. 
+    destruct (proj2 (H xs H6) X H0 sup_X H1 H5) as [x].
+    inversion H7; subst.
+    exists x...
+Qed.
+
+Next Obligation with eauto with *.
+  split.
+  - intros.
+    destruct H3...
+  - intros.
+    inversion H5; subst.
+    destruct (H2 X H3 sup_X H4 H6) as [x1].
+    destruct (H1 X H3 sup_X H4 H7) as [x2].
+    inversion H3; subst.
+    inversion H8; inversion H9; subst.
+    destruct (H11 x1 H12 x2 H17) as [x].
+    destruct H14.
+    destruct H15.
+    exists x...
+Qed.
+
+Definition U_x {D : Set} `{D_is_cpo : CompletePartialOrder D} : D -> Ensemble D :=
+  fun x : D => fun z : D => ~ leq z x
+.
+
+Lemma U_x_is_open {D : Set} `{D_is_cpo : CompletePartialOrder D} :
+  forall x : D,
+  is_open_set (U_x x).
+Proof with eauto with *.
+  intros x.
+  enough ( claim1 :
+    forall y : D,
+    forall z : D,
+    member y (U_x x) ->
+    leq y z ->
+    member z (U_x x)
+  ).
+  { split...
     intros.
-    induction H.
-    * exists n.
-      lia.
-    * destruct IHFinSet as [i].
-      exists i.
-      lia.
-  Qed.
-
-  Fixpoint FinSet_eqb {n1 : nat} {n2 : nat} (fs1 : FinSet n1) (fs2 : FinSet n2) : bool :=
-    match fs1 with
-    | FinSetZ _ =>
-      match fs2 with
-      | FinSetZ _ => true
-      | FinSetS _ fs2' => false 
-      end
-    | FinSetS _ fs1' =>
-      match fs2 with
-      | FinSetZ _ => false
-      | FinSetS _ fs2' => FinSet_eqb fs1' fs2'
-      end
-    end
-  .
-
-  End forFinSet.
-
-  Section forZip.
-
-  Fixpoint zip {A : Type} {B : Type} (xs : list A) (ys : list B) : list (A * B) :=
-    match xs, ys with
-    | x :: xs', y :: ys' => (x, y) :: zip xs' ys'
-    | _, _ => []
-    end
-  .
-
-  Lemma zip_main_property {A : Type} {B : Type} :
-    forall xs : list A,
-    forall ys : list B,
-    length xs = length ys ->
-    let zs : list (A * B) := zip xs ys in
-    map fst zs = xs /\ map snd zs = ys.
-  Proof.
-    intros xs.
-    induction xs.
-    - intros ys.
-      destruct ys.
-      * intros.
-        simpl.
-        tauto.
-      * intros.
-        inversion H.
-    - intros ys.
-      destruct ys.
-      * intros.
-        inversion H.
-      * intros.
-        inversion H.
-        assert (map fst (zip xs ys) = xs /\ map snd (zip xs ys) = ys).
-          apply IHxs.
-          tauto.
-        destruct H0.
-        unfold zs.
-        simpl.
-        rewrite H0.
-        rewrite H2.
-        tauto.
-  Qed.
-
-  Lemma zip_property1 {A : Type} {B : Type} :
-    forall zs : list (A * B),
-    zip (map fst zs) (map snd zs) = zs.
-  Proof.
-    intros zs.
-    induction zs.
-    - reflexivity.
-    - destruct a as [x y].
-      simpl.
-      rewrite IHzs.
-      reflexivity.
-  Qed.
-
-  End forZip.
-
-End AuxiliaPalatina.
-
-Module UntypedLambdaCalculus.
-
-  Import ListNotations.
-
-  Import AuxiliaPalatina.
-
-  Section Syntax.
-
-  Definition IVar : Set :=
-    nat
-  .
-
-  Lemma IVar_eq_dec :
-    forall x : IVar,
-    forall y : IVar,
-    {x = y} + {x <> y}.
-  Proof.
-    apply Nat.eq_dec.
-  Qed.
-
-  Inductive Term : Set :=
-  | Var :
-    forall x : IVar,
-    Term
-  | App :
-    forall P1 : Term,
-    forall P2 : Term,
-    Term
-  | Lam :
-    forall y : IVar,
-    forall Q : Term,
-    Term
-  .
-
-  Lemma Term_eq_dec :
-    forall M : Term,
-    forall N : Term,
-    {M = N} + {M <> N}.
-  Proof.
-    intros M.
-    induction M.
-    - intros N.
-      destruct N.
-      * destruct (IVar_eq_dec x x0).
-        { left.
-          subst.
-          reflexivity.
-        }
-        { right.
-          intro.
-          inversion H.
-          contradiction n.
-        }
-      * right.
-        intro.
-        inversion H.
-      * right.
-        intro.
-        inversion H.
-    - intros N.
-      destruct N.
-      * right.
-        intro.
-        inversion H.
-      * destruct (IHM1 N1).
-        { destruct (IHM2 N2).
-          { left.
-            subst.
-            reflexivity.
-          }
-          { right.
-            intro.
-            inversion H.
-            contradiction n.
-          }
-        }
-        { right.
-          intro.
-          inversion H.
-          contradiction n.
-        }
-      * right.
-        intro.
-        inversion H.
-    - intros N.
-      destruct N.
-      * right.
-        intro.
-        inversion H.
-      * right.
-        intro.
-        inversion H.
-      * destruct (IHM N).
-        { destruct (IVar_eq_dec y y0).
-          { left.
-            subst.
-            reflexivity.
-          }
-          { right.
-            intro.
-            inversion H.
-            contradiction n.
-          }
-        }
-        { right.
-          intro.
-          inversion H.
-          contradiction n.
-        }
-  Qed.
-
-  Inductive IsSubtermOf : Term -> Term -> Set :=
-  | IsSubtermOfRefl :
-    forall M : Term,
-    IsSubtermOf M M
-  | IsSubtermOfApp1 :
-    forall M : Term,
-    forall P1 : Term,
-    forall P2 : Term,
-    IsSubtermOf M P1 ->
-    IsSubtermOf M (App P1 P2)
-  | IsSubtermOfApp2 :
-    forall M : Term,
-    forall P1 : Term,
-    forall P2 : Term,
-    IsSubtermOf M P2 ->
-    IsSubtermOf M (App P1 P2)
-  | IsSubtermOfLam0 :
-    forall M : Term,
-    forall y : IVar,
-    forall Q : Term,
-    IsSubtermOf M Q ->
-    IsSubtermOf M (Lam y Q)
-  .
-
-  Fixpoint getRankOfTerm (M : Term) : nat :=
-    match M with
-    | Var x => 0
-    | App P1 P2 => S (max (getRankOfTerm P1) (getRankOfTerm P2))
-    | Lam y Q => S (getRankOfTerm Q)
-    end
-  .
-
-  Lemma getRankOfTerm_property1 :
-    forall M : Term,
-    forall N : Term,
-    IsSubtermOf M N ->
-    getRankOfTerm M <= getRankOfTerm N.
-  Proof.
-    intros.
-    induction H.
-    - lia.
-    - simpl.
-      lia.
-    - simpl.
-      lia.
-    - simpl.
-      lia.
-  Qed.
-
-  Lemma getRankOfTerm_property2 :
-    forall M : Term,
-    forall N : Term,
-    IsSubtermOf M N ->
-    getRankOfTerm M = getRankOfTerm N ->
-    M = N.
-  Proof.
-    intros M N X.
-    destruct X.
-    - tauto.
-    - assert (getRankOfTerm M <= getRankOfTerm P1).
-        apply getRankOfTerm_property1.
-        apply X.
-      simpl.
-      lia.
-    - assert (getRankOfTerm M <= getRankOfTerm P2).
-        apply getRankOfTerm_property1.
-        apply X.
-      simpl.
-      lia.
-    - assert (getRankOfTerm M <= getRankOfTerm Q).
-        apply getRankOfTerm_property1.
-        apply X.
-      simpl.
-      lia.
-  Qed.
-
-  Lemma IsSubtermOf_refl :
-    forall M : Term,
-    IsSubtermOf M M.
-  Proof.
-    apply IsSubtermOfRefl.
-  Qed.
-
-  Lemma IsSubtermOf_asym :
-    forall M : Term,
-    forall N : Term,
-    IsSubtermOf M N ->
-    IsSubtermOf N M ->
-    M = N.
-  Proof.
-    intros.
-    apply getRankOfTerm_property2.
-    apply H.
-    assert (getRankOfTerm M <= getRankOfTerm N).
-      apply getRankOfTerm_property1.
-      tauto.
-    assert (getRankOfTerm N <= getRankOfTerm M).
-      apply getRankOfTerm_property1.
-      tauto.
-    lia.
-  Qed.
-
-  Lemma IsSubtermOf_trans :
-    forall M : Term,
-    forall N : Term,
-    forall L : Term,
-    IsSubtermOf M N ->
-    IsSubtermOf N L ->
-    IsSubtermOf M L.
-  Proof.
-    cut (
-      forall L : Term,
-      forall N : Term,
-      forall M : Term,
-      IsSubtermOf M N ->
-      IsSubtermOf N L ->
-      IsSubtermOf M L
-    ).
-      intros.
-      apply (H L N M).
-      apply H0.
-      apply H1.
-    intros L.
-    induction L.
-    - intros N.
-      induction N.
-      * intros.
-        inversion H0.
-        { subst.
-          apply H.
-        }
-      * intros.
-        inversion H0.
-      * intros.
-        inversion H0.
-    - intros N.
-      induction N.
-      * intros.
-        inversion H0.
-        { subst.
-          apply IsSubtermOfApp1.
-          apply (IHL1 (Var x)).
-          apply H.
-          apply H3.
-        }
-        { subst.
-          apply IsSubtermOfApp2.
-          apply (IHL2 (Var x)).
-          apply H.
-          apply H3.
-        }
-      * intros.
-        inversion H.
-        { subst.
-          apply H0.
-        }
-        { subst.
-          inversion H0.
-          { subst.
-            apply H.
-          }
-          { subst.
-            apply IsSubtermOfApp1.
-            apply (IHL1 (App N1 N2)).
-            apply H.
-            apply H4.
-          }
-          { subst.
-            apply IsSubtermOfApp2.
-            apply (IHL2 (App N1 N2)).
-            apply H.
-            apply H4.
-          }
-        }
-        { subst.
-          inversion H0.
-          { subst.
-            apply H.
-          }
-          { subst.
-            apply IsSubtermOfApp1.
-            apply (IHL1 (App N1 N2)).
-            apply H.
-            apply H4.
-          }
-          { subst.
-            apply IsSubtermOfApp2.
-            apply (IHL2 (App N1 N2)).
-            apply H.
-            apply H4.
-          }
-        }
-      * intros.
-        inversion H.
-        { subst.
-          inversion H0.
-          { subst.
-            apply H0.
-          }
-          { subst.
-            apply H0.
-          }
-        }
-        { subst.
-          inversion H0.
-          { subst.
-            apply IsSubtermOfApp1.
-            apply (IHL1 (Lam y N)).
-            apply H.
-            apply H4.
-          }
-          { subst.
-            apply IsSubtermOfApp2.
-            apply (IHL2 (Lam y N)).
-            apply H.
-            apply H4.
-          }
-        }
-    - intros N.
-      induction N.
-      * intros.
-        inversion H.
-        { subst.
-          apply H0.
-        }
-      * intros.
-        inversion H.
-        { subst.
-          apply H0.
-        }
-        { subst.
-          inversion H0.
-          { subst.
-            apply IsSubtermOfLam0.
-            apply (IHL (App N1 N2)).
-            apply H.
-            apply H4.
-          } 
-        }
-        { subst.
-          inversion H0.
-          { subst.
-            apply IsSubtermOfLam0.
-            apply (IHL (App N1 N2)).
-            apply H.
-            apply H4.
-          }
-        }
-      * intros.
-        inversion H.
-        { subst.
-          apply H0.
-        }
-        { subst.
-          inversion H0.
-          { subst.
-            apply H.
-          }
-          { subst.
-            apply IsSubtermOfLam0.
-            apply (IHL (Lam y0 N)).
-            apply H.
-            apply H4.
-          }
-        }
-  Qed.
-
-  Theorem StrongInductionOnTerm (Phi : Term -> Prop) :
-    (forall M : Term, (forall N : Term, IsSubtermOf N M -> N <> M -> Phi N) -> Phi M) ->
-    forall M : Term,
-    Phi M.
-  Proof.
-    cut (
-      (forall M : Term, (forall N : Term, IsSubtermOf N M -> N <> M -> Phi N) -> Phi M) ->
-      forall M : Term,
-      forall N : Term,
-      IsSubtermOf N M ->
-      Phi N
-    ).
-    { intros.
-      apply (H H0 M M).
-      apply IsSubtermOf_refl.
+    inversion H; subst...
+    assert (claim2 : ~ (forall x0 : D, leq x0 x \/ ~ member x0 X)).
+    { intros H4.
+      contradiction H1.
+      unfold is_supremum in H0.
+      apply (proj2 (H0 x)).
+      intros x0 H5.
+      destruct (H4 x0)...
+      contradiction.
     }
-    intros XXX.
-    intros M.
-    induction M.
-    - intros.
-      apply XXX.
-      intros.
-      inversion H0.
-      * subst.
-        contradiction H1.
-        reflexivity.
-      * subst.
-        inversion H.
-      * subst.
-        inversion H.
-      * subst.
-        inversion H.
-    - intros.
-      apply XXX.
-      intros.
-      inversion H0.
-      * subst.
-        inversion H.
-        + subst.
-          contradiction H1.
-          reflexivity.
-        + subst.
-          apply IHM1.
-          apply H4.
-        + subst.
-          apply IHM2.
-          apply H4.
-      * subst.
-        inversion H.
-        + subst.
-          apply IHM1.
-          apply H2.
-        + subst.
-          apply IHM1.
-          apply (IsSubtermOf_trans N0 (App P1 P2)).
-          apply IsSubtermOfApp1.
-          apply H2.
-          apply H5.
-        + subst.
-          apply IHM2.
-          apply (IsSubtermOf_trans N0 (App P1 P2)).
-          apply IsSubtermOfApp1.
-          apply H2.
-          apply H5.
-      * subst.
-        inversion H.
-        + subst.
-          apply IHM2.
-          apply H2.
-        + subst.
-          apply IHM1.
-          apply (IsSubtermOf_trans N0 (App P1 P2)).
-          apply IsSubtermOfApp2.
-          apply H2.
-          apply H5.
-        + subst.
-          apply IHM2.
-          apply (IsSubtermOf_trans N0 (App P1 P2)).
-          apply IsSubtermOfApp2.
-          apply H2.
-          apply H5.
-      * subst.
-        inversion H.
-        + subst.
-          apply IHM1.
-          apply (IsSubtermOf_trans N0 (Lam y Q)).
-          apply H0.
-          apply H5.
-        + subst.
-          apply IHM2.
-          apply (IsSubtermOf_trans N0 (Lam y Q)).
-          apply H0.
-          apply H5.
-    - intros.
-      apply XXX.
-      intros.
-      inversion H0.
-      * subst.
-        contradiction H1.
-        reflexivity.
-      * subst.
-        inversion H.
-        + subst.
-          apply IHM.
-          apply (IsSubtermOf_trans N0 (App P1 P2)).
-          apply H0.
-          apply H5.
-      * subst.
-        inversion H.
-        + subst.
-          apply IHM.
-          apply (IsSubtermOf_trans N0 (App P1 P2)).
-          apply H0.
-          apply H5.
-      * subst.
-        inversion H.
-        + subst.
-          apply IHM.
-          apply H2.
-        + subst.
-          apply IHM.
-          apply (IsSubtermOf_trans N0 (Lam y0 Q)).
-          apply H0.
-          apply H5.
-  Qed.
+    apply not_all_ex_not in claim2.
+    destruct claim2 as [x1].
+    exists x1.
+    apply not_or_and in H4.
+    destruct H4.
+    apply NNPP in H5.
+    constructor...
+  }
+  unfold U_x, member.
+  intros y z H H0 H1.
+  contradiction H.
+  apply (transitivity (R:=leq) H0 H1).
+Qed.
 
-  Fixpoint isFreeIn (z : IVar) (M : Term) : bool :=
-    match M with
-    | Var x => if IVar_eq_dec x z then true else false
-    | App P1 P2 => isFreeIn z P1 || isFreeIn z P2
-    | Lam y Q => (if IVar_eq_dec y z then false else true) && isFreeIn z Q
-    end
-  .
+Definition characterization_of_continuous_map_on_cpos {D : Set} {D' : Set} `{D_is_cpo : CompletePartialOrder D} `{D'_is_cpo : CompletePartialOrder D'} : (D -> D') -> Prop :=
+  fun f : D -> D' =>
+  forall X : Ensemble D,
+  directed X ->
+  let Y : Ensemble D' := image f X in
+  exists sup_X : D, exists sup_Y : D', is_supremum sup_X X /\ is_supremum sup_Y Y /\ f sup_X =-= sup_Y
+.
 
-  Lemma isFreeIn_Var :
-    forall z : IVar,
-    forall x : IVar,
-    isFreeIn z (Var x) = true <-> x = z.
-  Proof.
-    intros.
-    simpl.
-    destruct (IVar_eq_dec x z).
-    - tauto.
-    - constructor.
-      * intros.
-        inversion H.
-      * intros.
-        contradiction n.
-  Qed.
+Lemma continuous_maps_on_cpos_are_always_monotonic {D : Set} {D' : Set} `{D_is_cpo : CompletePartialOrder D} `{D'_is_cpo : CompletePartialOrder D'} :
+  forall f : D -> D',
+  is_continuous_map f ->
+  forall x1 : D,
+  forall x2 : D,
+  leq x1 x2 ->
+  leq (f x1) (f x2).
+Proof with eauto with *.
+  intros f H x1 x2 H0.
+  apply NNPP.
+  intros H1.
+  assert (H2 : member (f x1) (U_x (f x2))) by now unfold U_x.
+  assert (H3 : member x1 (inverse_image f (U_x (f x2)))) by now constructor.
+  assert (H4 : is_open_set (inverse_image f (U_x (f x2)))) by now apply H, U_x_is_open.
+  assert (H5 : member x2 (inverse_image f (U_x (f x2)))) by now apply (proj1 H4 x1 x2).
+  enough (H6 : member (f x2) (U_x (f x2)))...
+  inversion H5...
+Qed.
 
-  Lemma isFreeIn_App :
-    forall z : IVar,
-    forall P1 : Term,
-    forall P2 : Term,
-    isFreeIn z (App P1 P2) = true <-> isFreeIn z P1 = true \/ isFreeIn z P2 = true.
-  Proof.
-    intros.
-    simpl.
-    rewrite orb_true_iff.
-    reflexivity.
-  Qed.
+Lemma property1_of_Scott_topology {D : Set} {D' : Set} `{D_is_cpo : CompletePartialOrder D} `{D'_is_cpo : CompletePartialOrder D'} :
+  forall f : D -> D',
+  is_continuous_map f ->
+  forall X : Ensemble D,
+  directed X ->
+  directed (image f X).
+Proof with eauto with *.
+  intros f H X H0.
+  destruct H0 as [H0 H1].
+  assert (H2 : forall x1 : D, forall x2 : D, leq x1 x2 -> leq (f x1) (f x2)) by now apply continuous_maps_on_cpos_are_always_monotonic.
+  split.
+  - destruct H0 as [x0]...
+  - intros y1 H3 y2 H4.
+    inversion H3; inversion H4; subst.
+    rename x into x1, x0 into x2.
+    destruct (H1 x1 H5 x2 H9) as [x3].
+    exists (f x3).
+    destruct H6.
+    destruct H7.
+    repeat split...
+Qed.
 
-  Lemma isFreeIn_Lam :
-    forall z : IVar,
-    forall y : IVar,
-    forall Q : Term,
-    isFreeIn z (Lam y Q) = true <-> y <> z /\ isFreeIn z Q = true.
-  Proof.
-    intros.
-    simpl.
-    rewrite andb_true_iff.
-    destruct (IVar_eq_dec y z).
-    - constructor.
-      * intros.
-        destruct H.
-        inversion H.
-      * intros.
-        destruct H.
-        contradiction H.
-    - tauto.
-  Qed.
+Lemma property2_of_Scott_topology {D : Set} {D' : Set} `{D_is_cpo : CompletePartialOrder D} `{D'_is_cpo : CompletePartialOrder D'} :
+  forall f : D -> D',
+  is_continuous_map f ->
+  forall X : Ensemble D,
+  directed X ->
+  forall sup_X : D,
+  is_supremum sup_X X ->
+  directed (image f X) ->
+  {sup_Y : D' | is_supremum sup_Y (image f X) /\ f sup_X =-= sup_Y}.
+Proof with eauto with *.
+  intros f H X H0 sup_X H1 H2.
+  set (Y := image f X).
+  assert (H3 : forall x1 : D, forall x2 : D, leq x1 x2 -> leq (f x1) (f x2)) by now apply continuous_maps_on_cpos_are_always_monotonic.
+  destruct (supremum_exists Y H2) as [sup_Y H4].
+  exists sup_Y.
+  assert (claim1 : leq sup_Y (f sup_X)).
+  { apply H4.
+    intros y H5.
+    inversion H5; subst.
+    apply H3, H1...
+  }
+  assert (claim2 : leq (f sup_X) sup_Y).
+  { apply NNPP.
+    intros H5.
+    assert (H6 : member (f sup_X) (U_x sup_Y)) by now unfold U_x.
+    assert (H7 : member sup_X (inverse_image f (U_x sup_Y))) by now constructor.
+    assert (H8 : is_open_set (inverse_image f (U_x sup_Y))) by now apply H, U_x_is_open.
+    destruct H8.
+    destruct (H9 X H0 sup_X H1 H7) as [x1].
+    inversion H10; subst.
+    inversion H12; subst.
+    contradiction H13.
+    apply H4...
+  }
+  split...
+Qed.
 
-  Definition Subst : Set :=
-    list (IVar * Term)
-  .
+Theorem the_main_reason_for_introducing_the_Scott_topology {D : Set} {D' : Set} `{D_is_cpo : CompletePartialOrder D} `{D'_is_cpo : CompletePartialOrder D'} :
+  forall f : D -> D',
+  is_continuous_map f <-> characterization_of_continuous_map_on_cpos f.
+Proof with eauto with *.
+  assert (claim1 : forall f : D -> D', is_continuous_map f -> forall x1 : D, forall x2 : D, leq x1 x2 -> leq (f x1) (f x2)) by apply continuous_maps_on_cpos_are_always_monotonic.
+  unfold characterization_of_continuous_map_on_cpos; split; intros H.
+  - intros X H0.
+    inversion H0; subst.
+    set (Y := image f X).
+    assert (H3 : directed Y) by now apply property1_of_Scott_topology.
+    destruct (supremum_exists X H0) as [sup_X H4].
+    exists sup_X.
+    destruct (property2_of_Scott_topology f H X H0 sup_X H4 H3) as [sup_Y H5].
+    exists sup_Y...
+  - assert (claim2 : forall x1 : D, forall x2 : D, leq x1 x2 -> leq (f x1) (f x2)).
+    { intros x1 x2 H0.
+      set (X := union (singleton x1) (singleton x2)).
+      set (Y := image f X).
+      assert (H1 : is_supremum x2 X).
+      { intros x.
+        split.
+        - intros H1 x' H2.
+          inversion H2; inversion H3; subst...
+        - intros H1.
+          apply H1...
+      }
+      assert (H2 : directed X).
+      { split.
+        - exists x1...
+        - intros x1' H2 x2' H3.
+          exists x2.
+          repeat split...
+          + inversion H2; (inversion H4; subst)...
+          + inversion H3; (inversion H4; subst)... 
+      }
+      destruct (H X H2) as [sup_X H3].
+      destruct H3 as [sup_Y H3].
+      destruct H3.
+      destruct H4.
+      assert (H6 : sup_X =-= x2) by now apply (supremum_unique X).
+      assert (H7 : sup_Y =-= f x2).
+      { apply (supremum_unique Y)...
+        intros y.
+        split...
+        intros H7 y' H8.
+        apply (leq_trans y' (f x2) y)...
+        apply H4...
+      }
+      apply H4...
+    }
+    intros O H0.
+    split.
+    + intros x1 x2 H1 H2.
+      inversion H1; subst.
+      constructor.
+      apply (proj1 H0 (f x1) (f x2))...
+    + intros X H1 sup_X H2 H3.
+      destruct (H X H1) as [sup_X' H4].
+      destruct H4 as [sup_Y H4].
+      destruct H4.
+      destruct H5.
+      assert (sup_X =-= sup_X') by now apply (supremum_unique X).
+      assert (H8 : member (f sup_X) O).
+      { inversion H3; subst...
+      }
+      assert (H9 : directed (image f X)).
+      { destruct H1.
+        split.
+        - destruct H1 as [x1].
+          exists (f x1)...
+        - intros y1 H10 y2 H11.
+          inversion H10; subst.
+          inversion H11; subst.
+          rename x into x1, x0 into x2.
+          destruct (H9 x1 H12 x2 H13) as [x3].
+          destruct H14.
+          destruct H15.
+          exists (f x3).
+          repeat split...
+      }
+      assert (H10 : NonEmpty (intersection (image f X) O)).
+      { apply (proj2 H0 (image f X) H9 (f sup_X))...
+        intros y.
+        split.
+        - intros.
+          apply H5...
+          apply (leq_trans sup_Y (f sup_X) y)...
+        - intros.
+          apply (leq_trans (f sup_X) sup_Y y)...
+          apply H5...
+      }
+      destruct H10 as [y1].
+      inversion H10; subst.
+      inversion H11; subst.
+      exists x...
+Qed.
 
-  Fixpoint runSubst_Var (sigma : Subst) (x : IVar) : Term :=
-    match sigma with
-    | [] => Var x
-    | (z, N) :: sigma' =>
-      if IVar_eq_dec x z
-      then N
-      else runSubst_Var sigma' x
-    end
-  .
-  End Syntax.
+Global Program Instance direct_product_of_two_poset_minor {D : Set} {D' : Set} `{D_is_poset_minor : Poset_minor D} `{D'_is_poset_minor : Poset_minor D'} : Poset_minor (D * D') :=
+  { eql := fun d1 : D * D' => fun d2 : D * D' => eql (fst d1) (fst d2) /\ eql (snd d1) (snd d2)
+  ; leq := fun d1 : D * D' => fun d2 : D * D' => leq (fst d1) (fst d2) /\ leq (snd d1) (snd d2)
+  }
+.
 
-  Lemma runSubst_Var_main_property :
-    forall sigma : Subst,
-    forall x : IVar,
-    forall M : Term,
-    runSubst_Var sigma x = M <-> (if In_dec IVar_eq_dec x (map fst sigma) then (exists sigma1 : Subst, exists sigma2 : Subst, sigma = sigma1 ++ [(x, M)] ++ sigma2 /\ ~ In x (map fst sigma1)) else Var x = M).
-  Proof.
-    intros sigma.
-    induction sigma.
-    - simpl.
-      intros.
-      tauto.
-    - destruct a as [x1 M1].
-      simpl.
-      intros.
-      destruct (IVar_eq_dec x x1).
-      * subst.
-        destruct (IVar_eq_dec x1 x1).
-        + constructor.
-          { intros.
-            exists [].
-            exists sigma.
-            simpl.
-            subst.
-            tauto.
-          }
-          { intros.
-            destruct H as [sigma1].
-            destruct H as [sigma2].
-            destruct H.
-            destruct sigma1.
-            - simpl in H.
-              inversion H.
-              subst.
-              reflexivity.
-            - simpl in H.
-              destruct p as [x2 M2].
-              inversion H.
-              subst.
-              contradiction H0.
-              simpl.
-              tauto.
-          }
-        + contradiction n.
-          reflexivity.
-      * destruct (IVar_eq_dec x1 x).
-        + contradiction n.
-          rewrite e.
-          reflexivity.
-        + rewrite IHsigma.
-          destruct (in_dec IVar_eq_dec x (map fst sigma)).
-          { simpl.
-            constructor.
-            - intros.
-              destruct H as [sigma1].
-              destruct H as [sigma2].
-              exists ((x1, M1) :: sigma1).
-              exists sigma2.
-              simpl.
-              destruct H.
-              constructor.
-              rewrite H.
-              reflexivity.
-              tauto.
-            - intros.
-              destruct H as [sigma1].
-              destruct H as [sigma2].
-              destruct H.
-              destruct sigma1.
-              * simpl in H.
-                inversion H.
-                subst.
-                contradiction n.
-                reflexivity.
-              * exists sigma1.
-                exists sigma2.
-                simpl in H.
-                inversion H.
-                subst.
-                constructor.
-                reflexivity.
-                simpl in H0.
-                tauto.
-          }
-          { reflexivity.
-          }
-  Qed.
+Next Obligation with eauto with *.
+  repeat split...
+  destruct H...
+  destruct H...
+  destruct H, H0.
+  apply (transitivity H H0).
+  destruct H, H0.
+  apply (transitivity H1 H2).
+Qed.
 
-  Lemma runSubst_Var_property1 :
-    forall sigma : Subst,
-    forall x : IVar,
-    forall M : Term,
-    runSubst_Var sigma x = M ->
-    (exists sigma1 : Subst, exists sigma2 : Subst, sigma = sigma1 ++ [(x, M)] ++ sigma2) \/ Var x = M.
-  Proof.
-    intros sigma.
-    induction sigma.
-    - simpl.
-      intros.
-      right.
-      apply H.
-    - destruct a as [x1 M1].
-      simpl.
-      intros.
-      destruct (IVar_eq_dec x x1).
-      * left.
-        exists [].
-        exists sigma.
-        simpl.
-        subst.
-        reflexivity.
-      * assert ((exists sigma1 sigma2 : Subst, sigma = sigma1 ++ [(x, M)] ++ sigma2) \/ Var x = M).
-          apply IHsigma.
-          apply H.
-        destruct H0.
-        + destruct H0 as [sigma1].
-          destruct H0 as [sigma2].
-          left.
-          exists ((x1, M1) :: sigma1).
-          exists sigma2.
-          simpl.
-          rewrite H0.
-          reflexivity.
-        + right.
-          apply H0.
-  Qed.
+Next Obligation with eauto with *.
+  repeat split...
+  destruct H, H0...
+  destruct H, H0...
+Qed.
 
-  Section Scoping.
+Next Obligation with eauto with *.
+  repeat split...
+  destruct H...
+  destruct H...
+  destruct H...
+  destruct H...
+  destruct H.
+  destruct H0, H...
+  destruct H.
+  destruct H0, H...
+Qed.
 
-  Fixpoint legio (Phi : IVar -> list IVar -> Prop) (M : Term) (Gamma : list IVar) : Prop :=
-    match M with
-    | Var x => Phi x Gamma
-    | App P1 P2 => legio Phi P1 Gamma /\ legio Phi P2 Gamma
-    | Lam y Q => legio Phi Q (y :: Gamma)
-    end
-  . 
+Global Program Instance direct_product_of_two_poset {D : Set} {D' : Set} `{D_is_poset : Poset D} `{D'_is_poset : Poset D'} : Poset (D * D') :=
+  {}
+.
 
-  Inductive OccursIn : IVar -> Term -> Set :=
-  | OccursInRefl :
-    forall x : IVar,
-    OccursIn x (Var x)
-  | OccursInApp1 :
-    forall x : IVar,
-    forall P1 : Term,
-    forall P2 : Term,
-    OccursIn x P1 ->
-    OccursIn x (App P1 P2)
-  | OccursInApp2 :
-    forall x : IVar,
-    forall P1 : Term,
-    forall P2 : Term,
-    OccursIn x P2 ->
-    OccursIn x (App P1 P2)
-  | OccursInLam0 :
-    forall x : IVar,
-    forall y : IVar,
-    forall Q : Term,
-    OccursIn x Q ->
-    OccursIn x (Lam y Q)
-  .
+Next Obligation with eauto with *.
+  constructor.
+  apply (substitutablity x1 x2 H (fun x : X => fst (f x))).
+  apply (substitutablity x1 x2 H (fun x : X => snd (f x))).
+Qed.
 
-  Fixpoint makeScope_aux (Gamma : list IVar) (x : IVar) (M : Term) (H : OccursIn x M) : list IVar :=
-    match H with
-    | OccursInRefl x => Gamma
-    | OccursInApp1 x P1 P2 H1 => makeScope_aux Gamma x P1 H1
-    | OccursInApp2 x P1 P2 H2 => makeScope_aux Gamma x P2 H2
-    | OccursInLam0 x y Q H0 => makeScope_aux (y :: Gamma) x Q H0
-    end
-  .
+Inductive getFsts {D : Set} {D' : Set} : Ensemble (D * D') -> Ensemble D :=
+| In_getFsts {ps : Ensemble (D * D')} :
+  forall x : D,
+  forall x' : D',
+  member (x, x') ps ->
+  member x (getFsts ps)
+.
 
-  Lemma legio_main_property (Phi : IVar -> list IVar -> Prop) :
-    forall M : Term,
-    forall Gamma : list IVar,
-    legio Phi M Gamma <-> (forall z : IVar, forall H : OccursIn z M, Phi z (makeScope_aux Gamma z M H)).
-  Proof.
-    assert ( claim1 :
-      forall M : Term,
-      forall z : IVar,
-      forall H : OccursIn z M,
-      forall Gamma : list IVar,
-      legio Phi M Gamma ->
-      Phi z (makeScope_aux Gamma z M H)
+#[global] Hint Constructors getFsts : domain_theory_hints.
+
+Inductive getSnds {D : Set} {D' : Set} : Ensemble (D * D') -> Ensemble D' :=
+| In_getSnds {ps : Ensemble (D * D')} :
+  forall x : D,
+  forall x' : D',
+  member (x, x') ps ->
+  member x' (getSnds ps)
+.
+
+#[global] Hint Constructors getSnds : domain_theory_hints.
+
+Program Instance direct_product_of_two_cpos {D : Set} {D' : Set} `{D_is_cpo : CompletePartialOrder D} `{D'_is_cpo : CompletePartialOrder D'} : CompletePartialOrder (D * D') :=
+  { bottom := (bottom, bottom)
+  }
+.
+
+Next Obligation with eauto with *.
+  split...
+Qed.
+
+Next Obligation with eauto with *.
+  assert (H0 : directed (getFsts xs)).
+  { destruct H.
+    split.
+    - destruct H.
+      exists (fst x).
+      apply (In_getFsts (fst x) (snd x)).
+      rewrite <- surjective_pairing...
+    - intros x1 H1 x2 H2.
+      inversion H1; subst.
+      rename x' into y1.
+      inversion H2; subst.
+      rename x' into y2.
+      destruct (H0 (x1, y1) H3 (x2, y2) H4) as [p].
+      destruct p as [x3 y3].
+      exists x3.
+      destruct H5.
+      destruct H6.
+      repeat split...
+      + apply H6.
+      + apply H7. 
+  }
+  assert (H1 : directed (getSnds xs)).
+  { destruct H.
+    split.
+    - destruct H.
+      exists (snd x).
+      apply (In_getSnds (fst x) (snd x)).
+      rewrite <- surjective_pairing...
+    - intros y1 H2 y2 H3.
+      inversion H2; subst.
+      rename x into x1.
+      inversion H3; subst.
+      rename x into x2.
+      destruct (H1 (x1, y1) H4 (x2, y2) H5) as [p].
+      destruct p as [x3 y3].
+      exists y3.
+      destruct H6.
+      destruct H7.
+      repeat split...
+      + apply H7.
+      + apply H8. 
+  }
+  destruct (supremum_exists (getFsts xs) H0) as [sup_fst_xs H2].
+  destruct (supremum_exists (getSnds xs) H1) as [sup_snd_xs H3].
+  exists (sup_fst_xs, sup_snd_xs).
+  intros p.
+  destruct p as [x y].
+  split.
+  - intros H4 p0 H5.
+    destruct p0 as [x0 y0].
+    split; [apply H2 | apply H3]...
+    all: apply H4.
+  - intros H4.
+    split; [apply H2 | apply H3]...
+    + intros x0 H5.
+      inversion H5; subst.
+      rename x' into y0.
+      apply (H4 (x0, y0))...
+    + intros y0 H5.
+      inversion H5; subst.
+      apply (H4 (x0, y0))...
+Defined.
+
+Local Notation "D1 ~> D2" := ({f : D1 -> D2 | is_continuous_map f}) (at level 15, right associativity) : type_scope.
+
+Lemma continuous_maps_are_continuous {D : Set} {D' : Set} `{D_is_cpo : CompletePartialOrder D} `{D'_is_cpo : CompletePartialOrder D'} :
+  forall f : D ~> D',
+  is_continuous_map (proj1_sig f).
+Proof.
+  apply proj2_sig.
+Qed.
+
+#[global] Hint Resolve continuous_maps_are_continuous : domain_theory_hints.
+
+Global Program Instance ContinuousMaps_is_Poset_minor {D : Set} {D' : Set} `{D_is_cpo : CompletePartialOrder D} `{D'_is_cpo : CompletePartialOrder D'} : Poset_minor (D ~> D') :=
+  { eql := fun f1 : D ~> D' => fun f2 : D ~> D' => forall x : D, eql (proj1_sig f1 x) (proj1_sig f2 x)
+  ; leq := fun f1 : D ~> D' => fun f2 : D ~> D' => forall x : D, leq (proj1_sig f1 x) (proj1_sig f2 x)
+  }
+.
+
+Next Obligation with eauto with *.
+  repeat split...
+  intros f1 f2 f3 H1 H2 x.
+  apply (transitivity (H1 x) (H2 x)).
+Qed.
+
+Next Obligation with eauto with *.
+  repeat split...
+Qed.
+
+Next Obligation with eauto with *.
+  intros f1 f2.
+  repeat split...
+  intros x.
+  apply leq_refl2...
+  intros H.
+  destruct H...
+Qed.
+
+Global Program Instance ContinuousMaps_is_Poset {D : Set} {D' : Set} `{D_is_cpo : CompletePartialOrder D} `{D'_is_cpo : CompletePartialOrder D'} : Poset (D ~> D') :=
+  {}
+.
+
+Next Obligation with eauto with *.
+  apply (substitutablity x1 x2 H (fun x' : X => proj1_sig (f x') x)).
+Qed.
+
+Lemma sup_of_maps_on_cpos_is_well_defined {D : Set} {D' : Set} `{D_is_cpo : CompletePartialOrder D} `{D'_is_cpo : CompletePartialOrder D'} :
+  forall fs : Ensemble (D ~> D'),
+  directed fs ->
+  forall x : D,
+  directed (image (fun f : D ~> D' => proj1_sig f x) fs).
+Proof with eauto with *.
+  intros fs H x.
+  destruct H.
+  split.
+  - destruct H as [f0].
+    exists (proj1_sig f0 x).
+    apply (In_image f0)...
+  - intros y1 H1 y2 H2.
+    inversion H1; subst.
+    inversion H2; subst.
+    rename x0 into f1, x1 into f2.
+    destruct (H0 f1 H3 f2 H4) as [f3].
+    destruct H5 as [H5 [H6 H7]].
+    exists (proj1_sig f3 x).
+    repeat split...
+    apply (In_image f3)...
+Qed.
+
+Lemma sup_of_continuous_maps_on_cpos_exists_if_their_set_is_directed {D : Set} {D' : Set} `{D_is_cpo : CompletePartialOrder D} `{D'_is_cpo : CompletePartialOrder D'} :
+  forall fs : Ensemble (D ~> D'),
+  forall directed_fs : directed fs,
+  let f : D -> D' := fun x : D => proj1_sig (supremum_exists (image (fun f_i : D ~> D' => proj1_sig f_i x) fs) (sup_of_maps_on_cpos_is_well_defined fs directed_fs x)) in
+  is_continuous_map f.
+Proof with eauto with *.
+  intros fs H f.
+  apply the_main_reason_for_introducing_the_Scott_topology.
+  intros X H0 Y.
+  destruct (supremum_exists X H0) as [sup_X H1].
+  exists sup_X, (f sup_X).
+  enough (is_supremum (f sup_X) Y)...
+  assert ( claim1 :
+    forall f_i : D ~> D',
+    member f_i fs ->
+    is_supremum (proj1_sig f_i sup_X) (image (fun x : D => proj1_sig f_i x) X)
+  ).
+  { intros f_i H2.
+    assert (H3 : is_continuous_map (proj1_sig f_i)) by now apply (proj2_sig f_i).
+    assert (H4 : characterization_of_continuous_map_on_cpos (proj1_sig f_i)) by now apply the_main_reason_for_introducing_the_Scott_topology.
+    destruct (H4 X H0) as [sup_X' [sup_Y' [H5 [H6 H7]]]].
+    assert (H8 : sup_X' =-= sup_X) by now apply (supremum_unique X).
+    apply (supremum_unique (image (fun x : D => proj1_sig f_i x) X) sup_Y' (proj1_sig f_i sup_X))...
+    symmetry.
+    transitivity (proj1_sig f_i sup_X')...
+  }
+  assert (claim2 : is_supremum (f sup_X) (image (fun f_i : D ~> D' => proj1_sig f_i sup_X) fs)) by apply (proj2_sig (supremum_exists (image (fun f_i : D ~> D' => proj1_sig f_i sup_X) fs) (sup_of_maps_on_cpos_is_well_defined fs H sup_X))).
+  set (sup_f_i_X_i := fun y : D' => exists f_i : D ~> D', member f_i fs /\ is_supremum y (image (fun x : D => proj1_sig f_i x) X)).
+  set (sup_x_X_f_i := fun y : D' => exists x : D, member x X /\ is_supremum y (image (fun f_i : D ~> D' => proj1_sig f_i x) fs)).
+  set (f_i_x := fun y : D' => exists f_i : D ~> D', exists x : D, member f_i fs /\ member x X /\ y =-= proj1_sig f_i x).
+  assert (claim3 : is_supremum (f sup_X) sup_f_i_X_i).
+  { intros y.
+    split.
+    - intros H2 y1 H3.
+      destruct H3 as [f1 [H3 H4]].
+      assert (H5 : is_supremum (proj1_sig f1 sup_X) (image (fun x : D => proj1_sig f1 x) X)) by now apply claim1.
+      assert (H6 : y1 =-= proj1_sig f1 sup_X) by now apply (supremum_unique (image (fun x : D => proj1_sig f1 x) X)).
+      apply (leq_trans y1 (proj1_sig f1 sup_X) y)...
+      apply (leq_trans (proj1_sig f1 sup_X) (f sup_X) y)...
+      apply claim2...
+      apply (In_image f1)...
+    - intros H2.
+      apply claim2...
+      intros y1 H3.
+      apply H2.
+      inversion H3; subst...
+      rename x into f1.
+      exists f1...
+  }
+  assert ( lemma1 :
+    forall sup : D',
+    is_supremum sup sup_f_i_X_i ->
+    is_supremum sup f_i_x
+  ).
+  { intros sup H2 y.
+    split.
+    - intros H3 y1 H4.
+      destruct H4 as [f1 [x1 [H4 [H5 H6]]]].
+      enough (H7 : forall x : D, forall x' : D, leq x x' -> leq (proj1_sig f1 x) (proj1_sig f1 x')).
+      { assert (H8 : leq (proj1_sig f1 x1) (proj1_sig f1 sup_X)) by now apply H7, H1.
+        apply (leq_trans y1 sup y)...
+        apply (leq_trans y1 (proj1_sig f1 x1) sup)...
+        apply (leq_trans (proj1_sig f1 x1) (proj1_sig f1 sup_X) sup)...
+        apply H2...
+        exists f1...
+      }
+      apply continuous_maps_on_cpos_are_always_monotonic...
+    - intros H3.
+      apply H2.
+      intros y1 [f1 [H4 H5]].
+      apply H5.
+      intros y' H6.
+      inversion H6; subst.
+      rename x into x1.
+      apply H3.
+      exists f1, x1...
+  }
+  assert ( lemma2 :
+    forall sup : D',
+    is_supremum sup f_i_x ->
+    is_supremum sup sup_x_X_f_i
+  ).
+  { intros sup H2 y.
+    split.
+    - intros H3 y1 [x1 [H4 H5]].
+      apply H5.
+      intros x' H6.
+      inversion H6; subst.
+      rename x into f1.
+      apply H2...
+      exists f1, x1...
+    - intros H3.
+      apply H2.
+      intros y1 [f1 [x1 [H4 [H5 H6]]]].
+      apply (leq_trans y1 (proj1_sig f1 x1) y)...
+      assert (H7 : is_supremum (f x1) (image (fun f_i : D ~> D' => proj1_sig f_i x1) fs)) by apply (proj2_sig (supremum_exists (image (fun f_i : D ~> D' => proj1_sig f_i x1) fs) (sup_of_maps_on_cpos_is_well_defined fs H x1))).
+      assert (H8 : leq (proj1_sig f1 x1) (f x1)).
+      { apply H7...
+        apply (In_image f1)...
+      }
+      apply (leq_trans (proj1_sig f1 x1) (f x1) y)...
+      apply H3...
+      assert (H9 : is_supremum (f x1) (image (fun f_i : D ~> D' => proj1_sig f_i x1) fs)) by apply (proj2_sig (supremum_exists (image (fun f_i : D ~> D' => proj1_sig f_i x1) fs) (sup_of_maps_on_cpos_is_well_defined fs H x1))).
+      exists x1...
+  }
+  enough (claim4 : is_supremum (f sup_X) sup_x_X_f_i).
+  { intros y.
+    split.  
+    - intros H2 y1 H3.
+      inversion H3; subst.
+      rename x into x1.
+      assert (H5 : is_supremum (f x1) (image (fun f_i : D ~> D' => proj1_sig f_i x1) fs)) by apply (proj2_sig (supremum_exists (image (fun f_i : D ~> D' => proj1_sig f_i x1) fs) (sup_of_maps_on_cpos_is_well_defined fs H x1))).
+      apply claim4...
+      exists x1...
+    - intros H2.
+      apply claim4...
+      intros y1 [x1 [H3 H4]].
+      assert (H5 : is_supremum (f x1) (image (fun f_i : D ~> D' => proj1_sig f_i x1) fs)) by apply (proj2_sig (supremum_exists (image (fun f_i : D ~> D' => proj1_sig f_i x1) fs) (sup_of_maps_on_cpos_is_well_defined fs H x1))).
+      assert (H6 : y1 =-= f x1) by now apply (supremum_unique (image (fun f_i : D ~> D' => proj1_sig f_i x1) fs) y1 (f x1)).
+      apply (leq_trans y1 (f x1) y)...
+  }
+  apply lemma2, lemma1...
+Qed.
+
+Definition supremum_of_continuous_maps {D : Set} {D' : Set} `{D_is_cpo : CompletePartialOrder D} `{D'_is_cpo : CompletePartialOrder D'} :
+  forall fs : Ensemble (D ~> D'),
+  directed fs ->
+  D ~> D'.
+Proof with eauto with *.
+  intros fs directed_fs.
+  exists (fun x : D => proj1_sig (supremum_exists (image (fun f_i : D ~> D' => proj1_sig f_i x) fs) (sup_of_maps_on_cpos_is_well_defined fs directed_fs x))).
+  apply sup_of_continuous_maps_on_cpos_exists_if_their_set_is_directed...
+Defined.
+
+Definition bottom_of_continuous_maps {D : Set} {D' : Set} `{D_is_cpo : CompletePartialOrder D} `{D'_is_cpo : CompletePartialOrder D'} :
+  D ~> D'.
+Proof with eauto with *.
+  exists (fun _ : D => bottom).
+  intros Y [H H0].
+  split.
+  - intros x1 x2 H1 H2.
+    inversion H1; subst...
+  - intros X [[x0 H1] H2] sup_X H3 H4.
+    exists x0.
+    constructor...
+    inversion H4; subst...
+Defined.
+
+Global Program Instance set_continuous_maps_on_cpos_is_cpo {D : Set} {D' : Set} `{D_is_cpo : CompletePartialOrder D} `{D'_is_cpo : CompletePartialOrder D'} : CompletePartialOrder (D ~> D') :=
+  { bottom := bottom_of_continuous_maps
+  }
+.
+
+Next Obligation with eauto with *.
+  apply bottom_least...
+Qed.
+
+Next Obligation with eauto with *.
+  rename xs into fs.
+  exists (supremum_of_continuous_maps fs H).
+  intros f.
+  split.
+  - intros H0 f0 H1 x.
+    apply (leq_trans (proj1_sig f0 x) (proj1_sig (supremum_of_continuous_maps fs H) x) (proj1_sig f x))...
+    assert (H2 : is_supremum (proj1_sig (supremum_of_continuous_maps fs H) x) (image (fun f_i : D ~> D' => proj1_sig f_i x) fs)) by now apply (proj2_sig (supremum_exists (image (fun f_i : D ~> D' => proj1_sig f_i x) fs) (sup_of_maps_on_cpos_is_well_defined fs H x))).
+    apply H2...
+    apply (In_image f0)...
+  - intros H0 x.
+    assert (H1 : is_supremum (proj1_sig (supremum_of_continuous_maps fs H) x) (image (fun f_i : D ~> D' => proj1_sig f_i x) fs)) by now apply (proj2_sig (supremum_exists (image (fun f_i : D ~> D' => proj1_sig f_i x) fs) (sup_of_maps_on_cpos_is_well_defined fs H x))).
+    apply H1...
+    intros y H2.
+    inversion H2; subst.
+    rename x0 into f0.
+    apply (H0 f0 H3 x).
+Defined.
+
+(* [PROVE ME] 2021-06-27:
+
+\begin{lstlisting}
+Lemma separately_continuous_iff {D1 : Set} {D2 : Set} {D3 : Set} `{D1_is_cpo : CompletePartialOrder D1} `{D2_is_cpo : CompletePartialOrder D2} `{D3_is_cpo : CompletePartialOrder D3} :
+  forall f : D1 * D2 -> D3,
+  is_continuous_map f <-> ((forall x1 : D1, is_continuous_map (fun x2 : D2 => f (x1, x2))) /\ (forall x2 : D2, is_continuous_map (fun x1 : D1 => f (x1, x2)))).
+\end{lstlisting}
+
+1.2.12 Lemma
+Let $f : D_1 \times D_2 \to D_3$.
+Then $f$ is continuous iff $f$ is continuous of its arguments separately.
+
+\begin{proof}
+  ($\Rightarrow$) Let $g = x_1 \mapsto f \left(x_1 , x_2 \right)$.
+    Then for directed $X \subseteq D_1$,
+    \begin{align*}
+      g \left( \sup X \right) 
+      & = f \left( \sup X , x_2 \right) \\
+      & = f \left( \sup \left\{ \left( x_1 , x_2 \right) | x_1 \in X \right\} \right) \\
+      & = \sup f \left( \left\{ \left( x_1 , x_2 \right) | x_1 \in X \right\} \right) \\
+      & = \sup g \left( X \right) .
+    \end{align*}
+    Hence $g$ is continuous and similarly $x_2 \mapsto f \left( x_1 , x_2 \right)$.
+  ($\Leftarrow$) Let $X \subseteq D_1 \times D_2$ be directed.
+    Then
+    \begin{align*}
+      f \left( \sup X \right)
+      & = f \left( \sup X_1 , \sup X_2 \right) \\
+      & = \sup_{x_1 \in X_1} f \left( x_1, X_2 \right) \\
+      & = \sup_{x_1 \in X_1} \sup_{x_2 \in X_2} f \left( x_1 , x_2 \right) \\
+      & = \sup_{\left( x_1 , x_2 \right) \in X} f \left( x_1 , x_2 \right) \\
+      & = \sup f \left( X \right)
+    \end{align*}
+    and so $f$ is continuous,
+    where $$ X_1 := \left\{ x_1 \in D_1 | \left( \exists x_2 \in D_2 \right) \left[ \left( x_1 , x_2 \right) \in X \right] \right\} ; $$ and $$ X_2 := \left\{ x_2 \in D_2 | \left( \exists x_1 \in D_1 \right) \left[ \left( x_1 , x_2 \right) \in X \right] \right\} . $$
+\end{proof}
+
+*)
+
+End DomainTheory.
+
+Module UntypedLamdbdaCalculus.
+
+Import ListNotations.
+
+Import AuxiliaryPalatina.
+
+Import DomainTheory.
+
+Definition ivar : Set :=
+  nat
+.
+
+Definition ivar_eq_dec :
+  forall x : ivar,
+  forall y : ivar,
+  {x = y} + {x <> y}.
+Proof.
+  apply Nat.eq_dec.
+Defined.
+
+Inductive tm : Set :=
+| tmVar : forall x : ivar, tm
+| tmApp : forall P1 : tm, forall P2 : tm, tm
+| tmLam : forall y : ivar, forall Q : tm, tm
+.
+
+Definition tm_eq_dec :
+  forall M1 : tm,
+  forall M2 : tm,
+  {M1 = M2} + {M1 <> M2}.
+Proof with try ((left; congruence) || (right; congruence)).
+  induction M1; destruct M2...
+  - destruct (ivar_eq_dec x x0)...
+  - destruct (IHM1_1 M2_1); destruct (IHM1_2 M2_2)...
+  - destruct (ivar_eq_dec y y0); destruct (IHM1 M2)...
+Defined.
+
+Section Subterm.
+
+Fixpoint getRank (M : tm) {struct M} : nat :=
+  match M with
+  | tmVar x => 0
+  | tmApp P1 P2 => S (max (getRank P1) (getRank P2))
+  | tmLam y Q => S (getRank Q)
+  end
+.
+
+Inductive subtm : tm -> tm -> Set :=
+| subtmRefl : forall M : tm, subtm M M
+| subtmAppL : forall M : tm, forall P1 : tm, forall P2 : tm, subtm M P1 -> subtm M (tmApp P1 P2)
+| subtmAppR : forall M : tm, forall P1 : tm, forall P2 : tm, subtm M P2 -> subtm M (tmApp P1 P2)
+| subtmLAbs : forall M : tm, forall y : ivar, forall Q : tm, subtm M Q -> subtm M (tmLam y Q)
+.
+
+Local Hint Constructors tm : core.
+
+Lemma subtm_getRank :
+  forall M : tm,
+  forall N : tm,
+  subtm M N ->
+  getRank M <= getRank N.
+Proof with lia.
+  intros M N X.
+  induction X; simpl...
+Qed.
+
+Lemma subtm_and_same_rank_implies_same_term :
+  forall M : tm,
+  forall N : tm,
+  subtm M N ->
+  getRank M = getRank N ->
+  M = N.
+Proof with lia.
+  intros M N X.
+  destruct X; intros.
+  - reflexivity.
+  - assert (H0 := subtm_getRank M P1 X).
+    simpl in *...
+  - assert (H0 := subtm_getRank M P2 X).
+    simpl in *...
+  - assert (H0 := subtm_getRank M Q X).
+    simpl in *...
+Qed.
+
+Lemma subtm_refl :
+  forall M1 : tm,
+  subtm M1 M1.
+Proof.
+  apply subtmRefl.
+Qed.
+
+Local Hint Resolve subtm_refl : core.
+
+Lemma subtm_asym :
+  forall M1 : tm,
+  forall M2 : tm,
+  subtm M1 M2 ->
+  subtm M2 M1 ->
+  M1 = M2.
+Proof with eauto.
+  intros.
+  apply subtm_and_same_rank_implies_same_term...
+  enough (getRank M1 <= getRank M2 /\ getRank M2 <= getRank M1) by lia.
+  split; apply subtm_getRank...
+Qed.
+
+Local Hint Resolve subtm_asym : core.
+
+Lemma subtm_trans :
+  forall M1 : tm,
+  forall M2 : tm,
+  forall M3 : tm,
+  subtm M1 M2 ->
+  subtm M2 M3 ->
+  subtm M1 M3.
+Proof with eauto.
+  enough (claim1 : forall L : tm, forall N : tm, forall M : tm, subtm N L -> subtm M N -> subtm M L)...
+  induction L.
+  all: intros; inversion H; subst...
+  - constructor 2...
+  - constructor 3...
+  - constructor 4...
+Qed.
+
+Local Hint Resolve subtm_trans : core.
+
+Theorem strong_induction_on_tm (phi : tm -> Prop) :
+  (forall M : tm, (forall N : tm, subtm N M -> N <> M -> phi N) -> phi M) ->
+  forall M : tm,
+  phi M.
+Proof with try now (firstorder; eauto).
+  intros XXX.
+  enough (claim1 : forall M : tm, forall L : tm, subtm L M -> phi L)...
+  induction M.
+  all: intros L H; apply XXX; intros N H0 H1; inversion H0; subst...
+  all: inversion H; subst...
+Qed.
+
+End Subterm.
+
+Section Occurences.
+
+Definition occurence_rect (XP : forall z : ivar, forall M : tm, subtm (tmVar z) M -> Type) :
+  (forall x : ivar, XP x (tmVar x) (subtmRefl (tmVar x))) ->
+  (forall x : ivar, forall P1 : tm, forall P2 : tm, forall X : subtm (tmVar x) P1, XP x P1 X -> XP x (tmApp P1 P2) (subtmAppL (tmVar x) P1 P2 X)) ->
+  (forall x : ivar, forall P1 : tm, forall P2 : tm, forall X : subtm (tmVar x) P2, XP x P2 X -> XP x (tmApp P1 P2) (subtmAppR (tmVar x) P1 P2 X)) ->
+  (forall x : ivar, forall y : ivar, forall Q : tm, forall X : subtm (tmVar x) Q, XP x Q X -> XP x (tmLam y Q) (subtmLAbs (tmVar x) y Q X)) ->
+  (forall x : ivar, forall M : tm, forall X : subtm (tmVar x) M, XP x M X).
+Proof.
+  intros XP_refl XP_appl XP_appr XP_labs z.
+  assert ( XXX :
+    forall N : tm,
+    forall M : tm,
+    forall X : subtm N M,
+    forall H : N = tmVar z,
+    XP z M (eq_rect N (fun N0 : tm => subtm N0 M) X (tmVar z) H)
+  ).
+  { assert ( XP_Refl :
+      forall M0 : tm,
+      forall H : M0 = tmVar z,
+      XP z M0 (eq_rect M0 (fun N1 : tm => subtm N1 M0) (subtmRefl M0) (tmVar z) H)
     ).
-    { intros M z H.
-      induction H.
-      - simpl.
-        tauto.
-      - simpl.
-        intros.
-        apply IHOccursIn.
-        apply H0.
-      - simpl.
-        intros.
-        apply IHOccursIn.
-        apply H0.
-      - simpl.
-        intros.
-        apply IHOccursIn.
-        apply H0.
+    { intros M0.
+      apply (case_eq M0 (tmVar z) (fun M1 : tm => fun H0 : M1 = tmVar z => XP z M1 (eq_rect M1 (fun N1 : tm => subtm N1 M1) (subtmRefl M1) (tmVar z) H0))).
+      apply (XP_refl z).
+    }
+    assert ( XP_AppL :
+      forall M0 : tm,
+      forall P1 : tm,
+      forall P2 : tm,
+      forall H : M0 = tmVar z,
+      forall X' : subtm M0 P1,
+      (forall H' : M0 = tmVar z, XP z P1 (eq_rect M0 (fun N1 : tm => subtm N1 P1) X' (tmVar z) H')) ->
+      XP z (tmApp P1 P2) (eq_rect M0 (fun N1 : tm => subtm N1 (tmApp P1 P2)) (subtmAppL M0 P1 P2 X') (tmVar z) H)
+    ).
+    { intros M0 P1 P2.
+      apply (case_eq M0 (tmVar z) (fun M1 : tm => fun H0 : M1 = tmVar z => forall X' : subtm M1 P1, (forall H' : M1 = tmVar z, XP z P1 (eq_rect M1 (fun N1 : tm => subtm N1 P1) X' (tmVar z) H')) -> XP z (tmApp P1 P2) (eq_rect M1 (fun N1 : tm => subtm N1 (tmApp P1 P2)) (subtmAppL M1 P1 P2 X') (tmVar z) H0))).
+      apply (fun X' : subtm (tmVar z) P1 => fun IHX' : forall H' : tmVar z = tmVar z, XP z P1 (eq_rect (tmVar z) (fun N1 : tm => subtm N1 P1) X' (tmVar z) H') => XP_appl z P1 P2 X' (IHX' eq_refl)).
+    }
+    assert ( XP_AppR :
+      forall M0 : tm,
+      forall P1 : tm,
+      forall P2 : tm,
+      forall H : M0 = tmVar z,
+      forall X' : subtm M0 P2,
+      (forall H' : M0 = tmVar z, XP z P2 (eq_rect M0 (fun N1 : tm => subtm N1 P2) X' (tmVar z) H')) ->
+      XP z (tmApp P1 P2) (eq_rect M0 (fun N1 : tm => subtm N1 (tmApp P1 P2)) (subtmAppR M0 P1 P2 X') (tmVar z) H)
+    ).
+    { intros M0 P1 P2.
+      apply (case_eq M0 (tmVar z) (fun M1 : tm => fun H0 : M1 = tmVar z => forall X' : subtm M1 P2, (forall H' : M1 = tmVar z, XP z P2 (eq_rect M1 (fun N1 : tm => subtm N1 P2) X' (tmVar z) H')) -> XP z (tmApp P1 P2) (eq_rect M1 (fun N1 : tm => subtm N1 (tmApp P1 P2)) (subtmAppR M1 P1 P2 X') (tmVar z) H0))).
+      apply (fun X' : subtm (tmVar z) P2 => fun IHX' : forall H' : tmVar z = tmVar z, XP z P2 (eq_rect (tmVar z) (fun N1 : tm => subtm N1 P2) X' (tmVar z) H') => XP_appr z P1 P2 X' (IHX' eq_refl)).
+    }
+    assert ( XP_LAbs :
+      forall M0 : tm,
+      forall y : ivar,
+      forall Q : tm,
+      forall H : M0 = tmVar z,
+      forall X' : subtm M0 Q,
+      (forall H' : M0 = tmVar z, XP z Q (eq_rect M0 (fun N1 : tm => subtm N1 Q) X' (tmVar z) H')) ->
+      XP z (tmLam y Q) (eq_rect M0 (fun N1 : tm => subtm N1 (tmLam y Q)) (subtmLAbs M0 y Q X') (tmVar z) H)
+    ).
+    { intros M0 y Q.
+      apply (case_eq M0 (tmVar z) (fun M1 : tm => fun H0 : M1 = tmVar z => forall X' : subtm M1 Q, (forall H' : M1 = tmVar z, XP z Q (eq_rect M1 (fun N1 : tm => subtm N1 Q) X' (tmVar z) H')) -> XP z (tmLam y Q) (eq_rect M1 (fun N1 : tm => subtm N1 (tmLam y Q)) (subtmLAbs M1 y Q X') (tmVar z) H0))).
+      apply (fun X' : subtm (tmVar z) Q => fun IHX' : forall H' : tmVar z = tmVar z, XP z Q (eq_rect (tmVar z) (fun N1 : tm => subtm N1 Q) X' (tmVar z) H') => XP_labs z y Q X' (IHX' eq_refl)).
+    }
+    apply (
+      fix occurence_rect_fix (N : tm) (M : tm) (X : subtm N M) {struct X} : forall H : N = tmVar z, XP z M (eq_rect N (fun N1 : tm => subtm N1 M) X (tmVar z) H) :=
+      match X as X0 in subtm N0 M0 return forall H : N0 = tmVar z, XP z M0 (eq_rect N0 (fun N1 : tm => subtm N1 M0) X0 (tmVar z) H) with
+      | subtmRefl M0 =>
+        fun H : M0 = tmVar z =>
+        XP_Refl M0 H 
+      | subtmAppL M0 P1 P2 X' =>
+        fun H : M0 = tmVar z =>
+        XP_AppL M0 P1 P2 H X' (occurence_rect_fix M0 P1 X')
+      | subtmAppR M0 P1 P2 X' =>
+        fun H : M0 = tmVar z =>
+        XP_AppR M0 P1 P2 H X' (occurence_rect_fix M0 P2 X')
+      | subtmLAbs M0 y Q X' =>
+        fun H : M0 = tmVar z =>
+        XP_LAbs M0 y Q H X' (occurence_rect_fix M0 Q X')
+      end
+    ).
+  }
+  apply (
+    fun M : tm =>
+    fun X : subtm (tmVar z) M =>
+    XXX (tmVar z) M X eq_refl
+  ).
+Defined.
+
+Fixpoint getFVs (M : tm) : list ivar :=
+  match M with
+  | tmVar x => [x]
+  | tmApp P1 P2 => getFVs P1 ++ getFVs P2
+  | tmLam y Q => remove ivar_eq_dec y (getFVs Q)
+  end
+.
+
+Fixpoint isFreeIn (z : ivar) (M : tm) {struct M} : bool :=
+  match M with
+  | tmVar x => Nat.eqb x z
+  | tmApp P1 P2 => isFreeIn z P1 || isFreeIn z P2
+  | tmLam y Q => isFreeIn z Q && negb (Nat.eqb z y)
+  end
+.
+
+Lemma getFVs_isFreeIn (M : tm) :
+  forall z : ivar,
+  In z (getFVs M) <-> isFreeIn z M = true.
+Proof with try now firstorder.
+  induction M; simpl; intros z.
+  - rewrite Nat.eqb_eq...
+  - rewrite orb_true_iff, in_app_iff...
+  - rewrite andb_true_iff, negb_true_iff, Nat.eqb_neq.
+    split; intros H.
+    + apply in_remove in H...
+    + apply in_in_remove...
+Qed.
+
+End Occurences.
+
+Section Substitution.
+
+Definition substitution : Set :=
+  ivar -> tm
+.
+
+Definition nil_subtitution : substitution :=
+  tmVar
+.
+
+Definition cons_substitution : ivar -> tm -> substitution -> substitution :=
+  fun x : ivar => fun M : tm => fun sigma : substitution => fun y : ivar => if ivar_eq_dec x y then M else sigma y
+.
+
+Fixpoint mk_substitution (sigma : list (ivar * tm)) {struct sigma} : substitution :=
+  match sigma with
+  | [] => nil_subtitution
+  | (x, M) :: sigma' => cons_substitution x M (mk_substitution sigma')
+  end
+.
+
+Definition get_max_ivar : tm -> ivar :=
+  fun M : tm => fold_right_max_0 (getFVs M)
+.
+
+Lemma get_max_ivar_lt (M : tm) :
+  forall x : ivar,
+  get_max_ivar M < x ->
+  isFreeIn x M = false.
+Proof with lia.
+  intros x.
+  enough (get_max_ivar M < x -> ~ In x (getFVs M)) by now rewrite getFVs_isFreeIn, not_true_iff_false in H.
+  assert (H1 : In x (getFVs M) -> fold_right_max_0 (getFVs M) >= x) by apply fold_right_max_0_in.
+  enough (fold_right_max_0 (getFVs M) >= x -> fold_right_max_0 (getFVs M) < x -> False) by now eauto...
+Qed.
+
+Definition isFreshIn_substitution : ivar -> substitution -> tm -> bool :=
+  fun x : ivar => fun sigma : substitution => fun M : tm => forallb (fun z : ivar => negb (isFreeIn x (sigma z))) (getFVs M)
+.
+
+Definition chi : substitution -> tm -> ivar :=
+  fun sigma : substitution => fun M : tm => S (fold_right_max_0 (map (fun x : ivar => get_max_ivar (sigma x)) (getFVs M)))
+.
+
+Theorem main_property_of_chi :
+  forall M : tm,
+  forall sigma : substitution,
+  isFreshIn_substitution (chi sigma M) sigma M = true.
+Proof with try now firstorder.
+  assert ( claim1 :
+    forall sigma : substitution,
+    forall M : tm,
+    forall x : ivar,
+    isFreeIn x M = true ->
+    isFreeIn (chi sigma M) (sigma x) = false
+  ).
+  { intros sigma M x H.
+    enough (get_max_ivar (sigma x) < chi sigma M) by now apply get_max_ivar_lt.
+    unfold chi, fold_right_max_0.
+    enough (fold_right max 0 (map (fun z : ivar => get_max_ivar (sigma z)) (getFVs M)) >= get_max_ivar (sigma x)) by lia.
+    rewrite <- getFVs_isFreeIn in H.
+    apply fold_right_max_0_in, in_map_iff...
+  }
+  unfold isFreshIn_substitution.
+  intros M sigma.
+  apply forallb_true_iff.
+  intros x H.
+  apply negb_true_iff, claim1, getFVs_isFreeIn...
+Qed.
+
+Lemma chi_nil : 
+  forall M : tm,
+  isFreeIn (chi nil_subtitution M) M = false.
+Proof with try now firstorder.
+  intros M.
+  assert (H : isFreshIn_substitution (chi nil_subtitution M) nil_subtitution M = true) by apply main_property_of_chi.
+  unfold isFreshIn_substitution in H.
+  rewrite forallb_true_iff in H.
+  simpl in H.
+  apply not_true_iff_false.
+  intros H0.
+  assert (H1 : negb (chi nil_subtitution M =? chi nil_subtitution M) = true) by now apply H, getFVs_isFreeIn.
+  rewrite negb_true_iff, Nat.eqb_neq in H1...
+Qed.
+
+Fixpoint run_substitution_on_tm (sigma : substitution) (M : tm) {struct M} : tm :=
+  match M with
+  | tmVar x => sigma x
+  | tmApp P1 P2 => tmApp (run_substitution_on_tm sigma P1) (run_substitution_on_tm sigma P2)
+  | tmLam y Q =>
+    let z : ivar := chi sigma M in
+    tmLam z (run_substitution_on_tm (cons_substitution y (tmVar z) sigma) Q)
+  end
+.
+
+Theorem main_property_isFreshIn_substitution :
+  forall M : tm,
+  forall z : ivar,
+  forall sigma : substitution,
+  isFreshIn_substitution z sigma M = true <-> isFreeIn z (run_substitution_on_tm sigma M) = false.
+Proof with try now firstorder.
+  induction M; simpl.
+  - intros z sigma.
+    unfold isFreshIn_substitution.
+    simpl.
+    rewrite andb_true_iff, negb_true_iff...
+  - intros z sigma.
+    rewrite orb_false_iff.
+    unfold isFreshIn_substitution.
+    simpl.
+    rewrite forallb_app, andb_true_iff...
+  - intros z sigma.
+    rewrite andb_false_iff, negb_false_iff, Nat.eqb_eq.
+    unfold isFreshIn_substitution.
+    simpl.
+    rewrite forallb_true_iff.
+    split; intros H.
+    + destruct (ivar_eq_dec z (chi sigma (tmLam y M)))...
+      left.
+      apply IHM.
+      unfold isFreshIn_substitution.
+      rewrite forallb_true_iff.
+      intros x H0.
+      unfold cons_substitution.
+      destruct (ivar_eq_dec y x).
+      * unfold isFreeIn.
+        apply negb_true_iff, Nat.eqb_neq...
+      * apply H, in_in_remove...
+    + intros x H0.
+      apply in_remove in H0.
+      destruct H0.
+      destruct H.
+      * assert (H2 : isFreshIn_substitution z (cons_substitution y (tmVar (chi sigma (tmLam y M))) sigma) M = true) by now apply IHM.
+        unfold isFreshIn_substitution in H2.
+        rewrite forallb_true_iff in H2.
+        assert (H3 := H2 x H0).
+        unfold cons_substitution in H3.
+        destruct (ivar_eq_dec y x)...
+      * assert (H2 : isFreshIn_substitution z sigma (tmLam y M) = true).
+        { rewrite H.
+          apply main_property_of_chi...
+        }
+        unfold isFreshIn_substitution in H2.
+        rewrite forallb_true_iff in H2.
+        apply H2.
+        rewrite getFVs_isFreeIn.
+        simpl.
+        rewrite andb_true_iff, negb_true_iff, Nat.eqb_neq, <- getFVs_isFreeIn...
+Qed.
+
+Definition equiv_substitution_wrt : substitution -> substitution -> tm -> Prop :=
+  fun sigma1 : substitution => fun sigma2 : substitution => fun M : tm => forall x : ivar, isFreeIn x M = true -> sigma1 x = sigma2 x
+.
+
+Lemma property1_of_equiv_substitution_wrt :
+  forall sigma1 : substitution,
+  forall sigma2 : substitution,
+  (forall x : ivar, sigma1 x = sigma2 x) ->
+  forall M : tm,
+  equiv_substitution_wrt sigma1 sigma2 M.
+Proof with try now firstorder.
+  unfold equiv_substitution_wrt...
+Qed.
+
+Lemma chi_equiv_substitution_wrt :
+  forall sigma1 : substitution,
+  forall sigma2 : substitution,
+  forall M : tm,
+  equiv_substitution_wrt sigma1 sigma2 M ->
+  chi sigma1 M = chi sigma2 M.
+Proof with reflexivity.
+  unfold chi.
+  intros sigma1 sigma2 M H.
+  enough (H0 : (map (fun x : ivar => get_max_ivar (sigma1 x)) (getFVs M)) = (map (fun x : ivar => get_max_ivar (sigma2 x)) (getFVs M))) by congruence.
+  apply map_ext_in.
+  intros x H0.
+  rewrite (H x (proj1 (getFVs_isFreeIn M x) H0))...
+Qed.
+
+Theorem main_property_of_equiv_substitution_wrt :
+  forall M : tm,
+  forall sigma1 : substitution,
+  forall sigma2 : substitution,
+  equiv_substitution_wrt sigma1 sigma2 M ->
+  run_substitution_on_tm sigma1 M = run_substitution_on_tm sigma2 M.
+Proof with try now firstorder.
+  induction M.
+  - intros sigma1 sigma2 H.
+    apply H.
+    simpl.
+    rewrite Nat.eqb_eq...
+  - intros sigma1 sigma2 H.
+    assert (H1 : equiv_substitution_wrt sigma1 sigma2 M1).
+    { intros x H0.
+      apply H.
+      simpl.
+      rewrite orb_true_iff...
+    }
+    assert (H2 : equiv_substitution_wrt sigma1 sigma2 M2).
+    { intros x H0.
+      apply H.
+      simpl.
+      rewrite orb_true_iff...
+    }
+    simpl.
+    rewrite (IHM1 sigma1 sigma2 H1), (IHM2 sigma1 sigma2 H2)...
+  - intros sigma1 sigma2 H.
+    simpl.
+    assert (H0 : equiv_substitution_wrt (cons_substitution y (tmVar (chi sigma1 (tmLam y M))) sigma1) (cons_substitution y (tmVar (chi sigma2 (tmLam y M))) sigma2) M).
+    { intros x H0.
+      unfold cons_substitution.
+      destruct (ivar_eq_dec y x).
+      - rewrite (chi_equiv_substitution_wrt sigma1 sigma2 (tmLam y M) H)...
+      - apply H.
+        simpl.
+        rewrite andb_true_iff, negb_true_iff, Nat.eqb_neq...
+    }
+    assert (H1 : chi sigma1 (tmLam y M) = chi sigma2 (tmLam y M)) by now apply chi_equiv_substitution_wrt.
+    rewrite (IHM (cons_substitution y (tmVar (chi sigma1 (tmLam y M))) sigma1) (cons_substitution y (tmVar (chi sigma2 (tmLam y M))) sigma2) H0), H1...
+Qed.
+
+Lemma trivial_substitution :
+  forall x : ivar,
+  forall M : tm,
+  run_substitution_on_tm (cons_substitution x (tmVar x) nil_subtitution) M = run_substitution_on_tm nil_subtitution M.
+Proof with try now firstorder.
+  unfold cons_substitution.
+  intros x M.
+  apply main_property_of_equiv_substitution_wrt.
+  intros y H.
+  destruct (ivar_eq_dec x y)...
+Qed.
+
+Definition compose_substitution : substitution -> substitution -> substitution :=
+  fun sigma1 : substitution => fun sigma2 : substitution => fun x : ivar => run_substitution_on_tm sigma1 (sigma2 x)
+.
+
+Lemma distri_compose_cons :
+  forall M : tm,
+  forall N : tm,
+  forall sigma1 : substitution,
+  forall sigma2 : substitution,
+  forall x : ivar,
+  forall y : ivar,
+  isFreshIn_substitution y sigma1 (tmLam x M) = true ->
+  forall z : ivar,
+  isFreeIn z M = true ->
+  cons_substitution x N (compose_substitution sigma2 sigma1) z = compose_substitution (cons_substitution y N sigma2) (cons_substitution x (tmVar y) sigma1) z.
+Proof with try now firstorder.
+  intros M N sigma1 sigma2 x y H z H0.
+  unfold cons_substitution, compose_substitution.
+  destruct (ivar_eq_dec x z).
+  - simpl.
+    destruct (ivar_eq_dec y y)...
+  - unfold isFreshIn_substitution in H.
+    rewrite forallb_true_iff in H.
+    assert (H1 : isFreeIn y (sigma1 z) = false).
+    { apply negb_true_iff, H, getFVs_isFreeIn.
+      simpl.
+      rewrite andb_true_iff, negb_true_iff, Nat.eqb_neq...
+    }
+    assert ( claim1 :
+      forall u : ivar,
+      isFreeIn u (sigma1 z) = true ->
+      cons_substitution y N sigma2 u = sigma2 u
+    ).
+    { unfold cons_substitution.
+      intros u H2.
+      destruct (ivar_eq_dec y u)...
+      subst.
+      rewrite H1 in H2...
+    }
+    apply main_property_of_equiv_substitution_wrt...
+Qed.
+
+Corollary distri_compose_cons_for_chi :
+  forall M : tm,
+  forall N : tm,
+  forall sigma1 : substitution,
+  forall sigma2 : substitution,
+  forall x : ivar,
+  let y : ivar := chi sigma1 (tmLam x M) in
+  forall z : ivar,
+  isFreeIn z M = true ->
+  cons_substitution x N (compose_substitution sigma2 sigma1) z = compose_substitution (cons_substitution y N sigma2) (cons_substitution x (tmVar y) sigma1) z.
+Proof with eauto using distri_compose_cons, main_property_of_chi.
+  intros M N sigma1 sigma2 x y z H...
+Qed.
+
+Definition FreeIn_wrt : ivar -> substitution -> tm -> Prop :=
+  fun x : ivar => fun sigma : substitution => fun M : tm => exists y : ivar, isFreeIn y M = true /\ isFreeIn x (sigma y) = true
+.
+
+Theorem isFreeIn_wrt_true_iff (M : tm) :
+  forall z : ivar,
+  forall sigma : substitution,
+  isFreeIn z (run_substitution_on_tm sigma M) = true <-> FreeIn_wrt z sigma M.
+Proof with try now firstorder.
+  unfold FreeIn_wrt.
+  induction M; simpl.
+  - intros z sigma.
+    split; intros H.
+    + exists x.
+      rewrite Nat.eqb_eq...
+    + destruct H as [y H].
+      rewrite Nat.eqb_eq in H.
+      destruct H.
+      subst...
+  - intros z sigma.
+    rewrite orb_true_iff.
+    split; intros H.
+    + destruct H; [enough (H0 : exists y : ivar, isFreeIn y M1 = true /\ isFreeIn z (sigma y) = true) | enough (H0 : exists y : ivar, isFreeIn y M2 = true /\ isFreeIn z (sigma y) = true)]...
+      all: destruct H0 as [y]; exists y; rewrite orb_true_iff...
+    + destruct H as [y].
+      rewrite orb_true_iff in H...
+  - intros x sigma.
+    rewrite andb_true_iff, negb_true_iff, Nat.eqb_neq.
+    split; intros H.
+    + destruct H.
+      assert (H1 := proj1 (IHM x (cons_substitution y (tmVar (chi sigma (tmLam y M))) sigma)) H).
+      destruct H1 as [w].
+      destruct H1.
+      set (z := chi sigma (tmLam y M)).
+      fold z in H, H0, H2.
+      destruct (ivar_eq_dec y w).
+      * subst.
+        unfold cons_substitution in H2.
+        destruct (ivar_eq_dec w w)...
+        unfold isFreeIn in H2.
+        rewrite Nat.eqb_eq in H2...
+      * exists w.
+        rewrite andb_true_iff, negb_true_iff, Nat.eqb_neq.
+        unfold cons_substitution in H2.
+        destruct (ivar_eq_dec y w)...
+    + rename y into z.
+      destruct H as [y].
+      destruct H.
+      set (w := chi sigma (tmLam z M)).
+      rewrite andb_true_iff, negb_true_iff, Nat.eqb_neq in H.
+      destruct (ivar_eq_dec w x).
+      * subst.
+        assert (isFreshIn_substitution w sigma (tmLam z M) = true) by now apply main_property_of_chi.
+        unfold isFreshIn_substitution in H1.
+        rewrite forallb_true_iff in H1.
+        enough (H2 : isFreeIn w (sigma y) = false) by now rewrite H0 in H2.
+        apply negb_true_iff, H1, getFVs_isFreeIn.
+        simpl.
+        rewrite andb_true_iff, negb_true_iff, Nat.eqb_neq...
+      * split...
+        apply IHM.
+        exists y.
+        split...
+        unfold cons_substitution.
+        destruct (ivar_eq_dec z y)...
+Qed.
+
+Lemma chi_ext :
+  forall sigma : substitution,
+  forall sigma' : substitution,
+  forall M : tm,
+  forall M' : tm,
+  (forall z : ivar, FreeIn_wrt z sigma M <-> FreeIn_wrt z sigma' M') ->
+  chi sigma M = chi sigma' M'.
+Proof with try now firstorder.
+  unfold chi, FreeIn_wrt.
+  intros.
+  enough (fold_right_max_0 (map (fun x : ivar => get_max_ivar (sigma x)) (getFVs M)) = fold_right_max_0 (map (fun x : ivar => get_max_ivar (sigma' x)) (getFVs M'))) by lia.
+  assert ( claim1 :
+    forall z : ivar,
+    In z (flat_map (fun y : ivar => getFVs (sigma y)) (getFVs M)) <-> In z (flat_map (fun y : ivar => getFVs (sigma' y)) (getFVs M'))
+  ).
+  { intros z.
+    repeat (rewrite in_flat_map).
+    split; intros.
+    all: destruct H0 as [x]; rewrite getFVs_isFreeIn in H0.
+    1: assert (H1 : exists y : ivar, isFreeIn y M' = true /\ isFreeIn z (sigma' y) = true).
+    3: assert (H1 : exists y : ivar, isFreeIn y M = true /\ isFreeIn z (sigma y) = true).
+    1, 3: apply H; exists x...
+    1, 2: rewrite getFVs_isFreeIn in H0...
+    all: destruct H1 as [y]; exists y; repeat (rewrite getFVs_isFreeIn)...
+  }
+  assert (H0 : fold_right_max_0 (flat_map (fun y : ivar => getFVs (sigma y)) (getFVs M)) = fold_right_max_0 (flat_map (fun y : ivar => getFVs (sigma' y)) (getFVs M'))) by now apply fold_right_max_0_ext.
+  unfold get_max_ivar.
+  enough (H1 : forall xs : list ivar, forall f : ivar -> list ivar, fold_right_max_0 (map (fun x : ivar => fold_right_max_0 (f x)) xs) = fold_right_max_0 (flat_map f xs)) by now repeat (rewrite H1).
+  induction xs; simpl; intros f...
+  rewrite fold_right_max_0_app...
+Qed.
+
+Theorem main_property_of_compose_substitution :
+  forall M : tm,
+  forall sigma1 : substitution,
+  forall sigma2 : substitution,
+  run_substitution_on_tm sigma2 (run_substitution_on_tm sigma1 M) = run_substitution_on_tm (compose_substitution sigma2 sigma1) M.
+Proof with try now firstorder.
+  induction M; simpl.
+  - intros sigma1 sigma2...
+  - intros sigma1 sigma2.
+    rewrite IHM1, IHM2...
+  - intros sigma1 sigma2.
+    enough (lemma : chi sigma2 (run_substitution_on_tm sigma1 (tmLam y M)) = chi (compose_substitution sigma2 sigma1) (tmLam y M)).
+    { set (x := chi sigma1 (tmLam y M)).
+      set (x' := chi sigma2 (tmLam x (run_substitution_on_tm (cons_substitution y (tmVar x) sigma1) M))).
+      set (z := chi (compose_substitution sigma2 sigma1) (tmLam y M)).
+      assert (H := IHM (cons_substitution y (tmVar x) sigma1) (cons_substitution x (tmVar x') sigma2)).
+      rewrite H.
+      assert (H0 : run_substitution_on_tm (compose_substitution (cons_substitution x (tmVar x') sigma2) (cons_substitution y (tmVar x) sigma1)) M = run_substitution_on_tm (cons_substitution y (tmVar x') (compose_substitution sigma2 sigma1)) M).
+      { apply main_property_of_equiv_substitution_wrt.
+        intros u H0.
+        assert (H1 := distri_compose_cons_for_chi M (tmVar x') sigma1 sigma2 y).
+        simpl in H1.
+        rewrite (H1 u H0)...
+      }
+      rewrite H0.
+      replace x' with z...
+    }
+    rename y into x.
+    set (y := chi sigma1 (tmLam x M)).
+    assert ( claim1 :
+      forall y' : ivar,
+      (exists x' : ivar, isFreeIn x' (tmLam y (run_substitution_on_tm (cons_substitution x (tmVar y) sigma1) M)) = true /\ isFreeIn y' (sigma2 x') = true) ->
+      (exists u : ivar, isFreeIn u (tmLam x M) = true /\ isFreeIn y' (compose_substitution sigma2 sigma1 u) = true)
+    ).
+    { intros y' H.
+      destruct H as [x'].
+      destruct H.
+      simpl in H.
+      rewrite andb_true_iff, negb_true_iff, Nat.eqb_neq in H.
+      destruct H.
+      assert (H2 := proj1 (isFreeIn_wrt_true_iff M x' (cons_substitution x (tmVar y) sigma1)) H).
+      destruct H2 as [u].
+      destruct H2.
+      unfold cons_substitution in H3.
+      destruct (ivar_eq_dec x u).
+      - unfold isFreeIn in H3.
+        rewrite Nat.eqb_eq in H3...
+      - exists u.
+        split.
+        + simpl.
+          rewrite andb_true_iff, negb_true_iff, Nat.eqb_neq...
+        + apply (proj2 (isFreeIn_wrt_true_iff (sigma1 u) y' sigma2))...
     }
     assert ( claim2 :
-      forall M : Term,
-      forall Gamma : list IVar,
-      (forall (z : IVar) (H : OccursIn z M), Phi z (makeScope_aux Gamma z M H)) ->
-      legio Phi M Gamma
+      forall y' : ivar,
+      (exists x' : ivar, isFreeIn x' (tmLam x M) = true /\ isFreeIn y' (compose_substitution sigma2 sigma1 x') = true) ->
+      (exists u : ivar, isFreeIn u (tmLam y (run_substitution_on_tm (cons_substitution x (tmVar y) sigma1) M)) = true /\ isFreeIn y' (sigma2 u) = true)
     ).
-    { intros M.
-      induction M.
-      - simpl.
-        intros.
-        apply (H x (OccursInRefl x)).
-      - simpl.
-        intros.
-        constructor.
-        { apply IHM1.
-          intros.
-          apply (H z (OccursInApp1 z M1 M2 H0)).
-        }
-        { apply IHM2.
-          intros.
-          apply (H z (OccursInApp2 z M1 M2 H0)).
-        }
-      - simpl.
-        intros.
-        apply IHM.
-        intros.
-        apply (H z (OccursInLam0 z y M H0)).
-    }
-    intros.
-    constructor.
-    - intros.
-      apply claim1.
-      apply H.
-    - intros.
-      apply claim2.
-      apply H.
-  Qed.
-
-  End Scoping.
-
-  Section DeBruijn.
-
-  Fixpoint getDeBruijnIndex (Gamma : list IVar) (z : IVar) : option nat :=
-    match Gamma with
-    | [] => None
-    | x :: Gamma' => 
-      if IVar_eq_dec x z
-      then Some 0
-      else
-      match getDeBruijnIndex Gamma' z with
-      | None => None
-      | Some n => Some (S n)
-      end
-    end
-  .
-
-  Lemma getDeBruijnIndex_property1 :
-    forall Gamma : list IVar,
-    forall z : IVar,
-    getDeBruijnIndex Gamma z = None <-> ~ In z Gamma.
-  Proof.
-    intros Gamma.
-    induction Gamma.
-    - intros.
-      simpl.
-      tauto.
-    - intros.
-      simpl.
-      destruct (IVar_eq_dec a z).
-      * constructor.
-        + intros.
-          inversion H.
-        + intros.
-          contradiction H.
-          tauto.
-      * assert (getDeBruijnIndex Gamma z = None <-> ~ In z Gamma).
-          apply IHGamma.
-        constructor.
-        + intros.
-          destruct (getDeBruijnIndex Gamma z).
-          { inversion H0.
-          }
-          { tauto.
-          }
-        + intros.
-          destruct (getDeBruijnIndex Gamma z).
-          { contradiction H0.
-            right.
-            assert (~ Some n0 = None).
-              intro.
-              inversion H1.
-            tauto.
-          }
-          { reflexivity.
-          }
-  Qed.
-
-  Lemma getDeBruijnIndex_property2 :
-    forall Gamma : list IVar,
-    forall z : IVar,
-    In z Gamma ->
-    exists idx : nat, getDeBruijnIndex Gamma z = Some idx.
-  Proof.
-    intros Gamma.
-    induction Gamma.
-    - intros.
-      inversion H.
-    - intros.
+    { intros y' H.
+      destruct H as [x'].
+      destruct H.
       simpl in H.
-      destruct (IVar_eq_dec a z).
-      * exists 0.
-        simpl.
-        destruct (IVar_eq_dec a z).
-        + reflexivity.
-        + contradiction n.
-      * assert (In z Gamma).
-          tauto.
-        destruct (IHGamma z H0) as [idx].
-        exists (S idx).
-        simpl.
-        rewrite H1.
-        destruct (IVar_eq_dec a z).
-        + contradiction n.
-        + reflexivity.
-  Qed.
-
-  Lemma getDeBruijnIndex_property3 :
-    forall Gamma : list IVar,
-    forall z : IVar,
-    forall idx : nat,
-    getDeBruijnIndex Gamma z = Some idx -> 
-    exists Gamma1 : list IVar,
-    exists Gamma2 : list IVar,
-    ((Gamma = Gamma1 ++ [z] ++ Gamma2 /\ length Gamma1 = idx) /\ (forall x : IVar, In x Gamma1 -> x <> z)).
-  Proof.
-    intros Gamma.
-    induction Gamma.
-    - simpl.
-      intros.
-      inversion H.
-    - simpl.
-      intros.
-      destruct (IVar_eq_dec a z).
-      * inversion H.
-        subst.
-        exists [].
-        exists Gamma.
-        constructor.
-        + tauto.
-        + intros.
-          inversion H0.
-      * assert (
-          forall idx : IVar,
-          getDeBruijnIndex Gamma z = Some idx ->
-          exists Gamma1 : list IVar,
-          exists Gamma2 : list IVar,
-          (Gamma = Gamma1 ++ [z] ++ Gamma2 /\ length Gamma1 = idx) /\ (forall x : IVar, In x Gamma1 -> x <> z)
-        ).
-          apply IHGamma.
-        destruct (getDeBruijnIndex Gamma z).
-        + inversion H.
-          subst.
-          assert (
-            exists Gamma1 : list IVar,
-            exists Gamma2 : list IVar,
-            (Gamma = Gamma1 ++ [z] ++ Gamma2 /\ length Gamma1 = n0) /\ (forall x : IVar, In x Gamma1 -> x <> z)
-          ).
-            apply H0.
-            reflexivity.
-          destruct H1 as [Gamma1].
-          destruct H1 as [Gamma2].
-          destruct H1.
-          destruct H1.
-          exists (a :: Gamma1).
-          exists Gamma2.
-          constructor.
-          constructor.
-          rewrite H1.
-          simpl.
-          reflexivity.
-          simpl.
-          rewrite H3.
-          reflexivity.
-          intros.
-          simpl in H4.
-          destruct H4.
-          subst.
-          apply n.
-          apply H2.
-          apply H4.
-        + inversion H.
-  Qed.
-
-  Inductive DeBruijnTerm : Set :=
-  | BVar : nat -> DeBruijnTerm
-  | FVar : IVar -> DeBruijnTerm
-  | IApp : DeBruijnTerm -> DeBruijnTerm -> DeBruijnTerm
-  | IAbs : DeBruijnTerm -> DeBruijnTerm
-  .
-
-  Fixpoint makeDeBruijnTerm_aux (Gamma : list IVar) (M : Term) : DeBruijnTerm :=
-    match M with
-    | Var x =>
-      match getDeBruijnIndex Gamma x with
-      | None => FVar x
-      | Some idx => BVar idx
-      end
-    | App P1 P2 => IApp (makeDeBruijnTerm_aux Gamma P1) (makeDeBruijnTerm_aux Gamma P2)
-    | Lam y Q => IAbs (makeDeBruijnTerm_aux (y :: Gamma) Q)
-    end
-  .
-
-  Inductive mapsToDeBruijn : list IVar -> Term -> DeBruijnTerm -> Prop :=
-  | mapsToDeBruijnBVar :
-    forall Gamma : list IVar,
-    forall x : IVar,
-    forall idx : nat,
-    getDeBruijnIndex Gamma x = Some idx ->
-    mapsToDeBruijn Gamma (Var x) (BVar idx)
-  | mapsToDeBruijnFVar :
-    forall Gamma : list IVar,
-    forall x : IVar,
-    getDeBruijnIndex Gamma x = None ->
-    mapsToDeBruijn Gamma (Var x) (FVar x)
-  | mapsToDeBruijnIApp :
-    forall Gamma : list IVar,
-    forall P1 : Term,
-    forall P2 : Term,
-    forall P1' : DeBruijnTerm,
-    forall P2' : DeBruijnTerm,
-    mapsToDeBruijn Gamma P1 P1' ->
-    mapsToDeBruijn Gamma P2 P2' ->
-    mapsToDeBruijn Gamma (App P1 P2) (IApp P1' P2')
-  | mapsToDeBruijnIAbs :
-    forall Gamma : list IVar,
-    forall y : IVar,
-    forall Q : Term,
-    forall Q' : DeBruijnTerm,
-    mapsToDeBruijn (y :: Gamma) Q Q' ->
-    mapsToDeBruijn Gamma (Lam y Q) (IAbs Q')
-  .
-
-  Lemma makeDeBruijnTerm_aux_main_property :
-    forall M : Term,
-    forall M' : DeBruijnTerm,
-    forall Gamma : list IVar,
-    M' = makeDeBruijnTerm_aux Gamma M <-> mapsToDeBruijn Gamma M M'.
-  Proof.
-    intros M.
-    induction M.
-    - intros.
+      rewrite andb_true_iff, negb_true_iff, Nat.eqb_neq in H.
+      destruct H.
+      assert (H2 := proj1 (isFreeIn_wrt_true_iff (sigma1 x') y' sigma2) H0).
+      destruct H2 as [u].
+      destruct H2.
+      assert (H4 : isFreeIn u (run_substitution_on_tm (cons_substitution x (tmVar y) sigma1) M) = true).
+      { apply isFreeIn_wrt_true_iff.
+        exists x'.
+        split...
+        unfold cons_substitution.
+        destruct (ivar_eq_dec x x')...
+      }
+      exists u.
+      split...
       simpl.
-      cut (
-        let idx' : option nat := getDeBruijnIndex Gamma x in
-        idx' = getDeBruijnIndex Gamma x ->
-        M' = (match idx' with | Some idx => BVar idx | None => FVar x end) <-> mapsToDeBruijn Gamma (Var x) M'
-      ).
-        intros.
-        apply H.
-        reflexivity.
-      intros.
-      destruct idx'.
-      * constructor.
-        + intros.
-          subst.
-          apply (mapsToDeBruijnBVar Gamma x n).
-          rewrite H.
-          reflexivity.
-        + intros.
-          inversion H0.
-          { subst.
-            rewrite H3 in H.
-            inversion H.
-            subst.
-            reflexivity.
-          }
-          { subst.
-            rewrite H3 in H.
-            inversion H.
-          }
-      * constructor.
-        + intros.
-          subst.
-          apply (mapsToDeBruijnFVar Gamma x).
-          rewrite H.
-          reflexivity.
-        + intros.
-          inversion H0.
-          { subst.
-            rewrite H3 in H.
-            inversion H.
-          }
-          { subst.
-            rewrite H3 in H.
-            inversion H.
-            subst.
-            reflexivity.
-          }
-    - intros.
-      constructor.
-      * intros.
-        subst.
-        simpl.
-        apply mapsToDeBruijnIApp.
-        apply IHM1.
-        reflexivity.
-        apply IHM2.
-        reflexivity.
-      * intros.
-        inversion H.
-        subst.
-        simpl.
-        assert (P1' = makeDeBruijnTerm_aux Gamma M1).
-          apply IHM1.
-          apply H3.
-        assert (P2' = makeDeBruijnTerm_aux Gamma M2).
-          apply IHM2.
-          apply H5.
-        rewrite H0.
-        rewrite H1.
-        reflexivity.
-    - intros.
-      constructor.
-      * intros.
-        subst.
-        simpl.
-        apply mapsToDeBruijnIAbs.
-        apply IHM.
-        reflexivity.
-      * intros.
-        inversion H.
-        subst.
-        simpl.
-        assert (Q' = makeDeBruijnTerm_aux (y :: Gamma) M).
-          apply IHM.
-          apply H4.
-        rewrite H0.
-        reflexivity.
-  Qed.
+      rewrite andb_true_iff, negb_true_iff, Nat.eqb_neq.
+      split...
+      intros H5.
+      subst.
+      enough (H6 : isFreeIn y (sigma1 x') = false) by now rewrite H2 in H6.
+      assert (H5 := main_property_of_chi (tmLam x M) sigma1).
+      unfold isFreshIn_substitution in H5.
+      rewrite forallb_true_iff in H5.
+      apply negb_true_iff, H5.
+      rewrite getFVs_isFreeIn.
+      simpl.
+      rewrite andb_true_iff, negb_true_iff, Nat.eqb_neq...
+    }
+    apply chi_ext...
+Qed.
 
-  Definition makeDeBruijnTerm : Term -> DeBruijnTerm :=
-    makeDeBruijnTerm_aux []
-  .
+Corollary compose_one :
+  forall M : tm,
+  forall N : tm,
+  forall sigma : substitution,
+  forall x : ivar,
+  run_substitution_on_tm (cons_substitution x (run_substitution_on_tm sigma N) sigma) M = run_substitution_on_tm sigma (run_substitution_on_tm (cons_substitution x N nil_subtitution) M).
+Proof with try now firstorder.
+  intros M N sigma x.
+  replace (run_substitution_on_tm (cons_substitution x (run_substitution_on_tm sigma N) sigma) M) with (run_substitution_on_tm (cons_substitution x (run_substitution_on_tm sigma N) (compose_substitution sigma nil_subtitution)) M).
+  replace (run_substitution_on_tm (cons_substitution x (run_substitution_on_tm sigma N) (compose_substitution sigma nil_subtitution)) M) with (run_substitution_on_tm (compose_substitution sigma (cons_substitution x N nil_subtitution)) M).
+  rewrite main_property_of_compose_substitution...
+  all: apply main_property_of_equiv_substitution_wrt; apply property1_of_equiv_substitution_wrt; unfold compose_substitution, cons_substitution, nil_subtitution; intros z; destruct (ivar_eq_dec x z)...
+Qed.
 
-  End DeBruijn.
+Theorem main_property_of_cons_substitution :
+  forall x : ivar,
+  forall z : ivar,
+  forall M : tm,
+  forall N : tm,
+  forall sigma : substitution,
+  isFreeIn z (tmLam x M) = false ->
+  run_substitution_on_tm (cons_substitution x N sigma) M = run_substitution_on_tm (cons_substitution z N sigma) (run_substitution_on_tm (cons_substitution x (tmVar z) nil_subtitution) M).
+Proof with try now firstorder.
+  intros.
+  rewrite (main_property_of_compose_substitution M (cons_substitution x (tmVar z) nil_subtitution) (cons_substitution z N sigma)).
+  apply main_property_of_equiv_substitution_wrt.
+  intros w H0.
+  unfold cons_substitution, nil_subtitution, compose_substitution.
+  destruct (ivar_eq_dec x w); simpl.
+  - destruct (ivar_eq_dec z z)...
+  - destruct (ivar_eq_dec z w)...
+    simpl in H.
+    subst.
+    rewrite H0 in H.
+    simpl in H.
+    rewrite negb_false_iff, Nat.eqb_eq in H.
+    contradiction n...
+Qed.
 
-  Section AlphaEquiv.
+End Substitution.
 
-  End AlphaEquiv.
+#[global] Create HintDb semantics_of_ulc.
 
-End UntypedLambdaCalculus.
+Class isPreLambdaStructure (Dom : Set) : Type :=
+  { eqnDom : Dom -> Dom -> Prop
+  ; runApp : Dom -> (Dom -> Dom)
+  ; runLam : (Dom -> Dom) -> Dom
+  ; eqnDom_refl :
+    forall v1 : Dom,
+    eqnDom v1 v1
+  ; eqnDom_sym :
+    forall v1 : Dom,
+    forall v2 : Dom,
+    eqnDom v1 v2 ->
+    eqnDom v2 v1
+  ; eqnDom_trans :
+    forall v1 : Dom,
+    forall v2 : Dom,
+    forall v3 : Dom,
+    eqnDom v1 v2 ->
+    eqnDom v2 v3 ->
+    eqnDom v1 v3
+  ; runApp_ext :
+    forall v1 : Dom,
+    forall v1' : Dom,
+    forall v2 : Dom,
+    forall v2' : Dom,
+    eqnDom v1 v1' ->
+    eqnDom v2 v2' ->
+    eqnDom (runApp v1 v2) (runApp v1' v2')
+  ; runLam_ext :
+    forall vv : Dom -> Dom,
+    forall vv' : Dom -> Dom,
+    (forall v0 : Dom, eqnDom (vv v0) (vv' v0)) ->
+    eqnDom (runLam vv) (runLam vv')
+  }
+.
+
+Local Notation "v1 =-= v2" := (eqnDom v1 v2) (at level 70, no associativity) : type_scope.
+
+#[global] Hint Resolve eqnDom_refl : semantics_of_ulc.
+
+#[global] Hint Resolve eqnDom_sym : semantics_of_ulc.
+
+#[global] Hint Resolve eqnDom_trans : semantics_of_ulc.
+
+#[global] Hint Resolve runApp_ext : semantics_of_ulc.
+
+#[global] Hint Resolve runLam_ext : semantics_of_ulc.
+
+Section PreLambdaStructure.
+
+Variable D : Set.
+
+Fixpoint eval_tm `{D_is_model : isPreLambdaStructure D} (E : ivar -> D) (M : tm) {struct M} : D :=
+  match M with
+  | tmVar x => E x
+  | tmApp P1 P2 => runApp (eval_tm E P1) (eval_tm E P2)
+  | tmLam y Q => runLam (fun v : D => eval_tm (fun z : ivar => if ivar_eq_dec y z then v else E z) Q)
+  end
+.
+
+Lemma eval_tm_ext `{D_is_model : isPreLambdaStructure D} :
+  forall M : tm,
+  forall E1 : ivar -> D,
+  forall E2 : ivar -> D,
+  (forall z : ivar, isFreeIn z M = true -> E1 z =-= E2 z) ->
+  eval_tm E1 M =-= eval_tm E2 M.
+Proof with try now firstorder with semantics_of_ulc.
+  induction M; simpl.
+  - intros E1 E2 H.
+    apply H.
+    rewrite Nat.eqb_eq...
+  - intros E1 E2 H.
+    apply runApp_ext; [apply IHM1 | apply IHM2].
+    all: intros z H0; apply H; rewrite orb_true_iff...
+  - intros E1 E2 H.
+    apply runLam_ext.
+    intros v.
+    apply (IHM (fun z : ivar => if ivar_eq_dec y z then v else E1 z) (fun z : ivar => if ivar_eq_dec y z then v else E2 z))...
+    intros z H0.
+    destruct (ivar_eq_dec y z)...
+    apply H.
+    rewrite andb_true_iff, negb_true_iff, Nat.eqb_neq...
+Qed.
+
+Theorem run_substitution_on_tm_preserves_eval_tm `{D_is_model : isPreLambdaStructure D} :
+  forall M : tm,
+  forall sigma : substitution,
+  forall E : ivar -> D,
+  eval_tm (fun z : ivar => eval_tm E (sigma z)) M =-= eval_tm E (run_substitution_on_tm sigma M).
+Proof with try now firstorder with semantics_of_ulc.
+  induction M.
+  - intros sigma E...
+  - intros sigma E.
+    simpl...
+  - intros sigma E.
+    enough (claim1 : forall v : D, eval_tm (fun z : ivar => if ivar_eq_dec y z then v else eval_tm E (sigma z)) M =-= eval_tm (fun z : ivar => if ivar_eq_dec (chi sigma (tmLam y M)) z then v else E z) (run_substitution_on_tm (cons_substitution y (tmVar (chi sigma (tmLam y M))) sigma) M)) by now apply runLam_ext.
+    intros v.
+    assert (H := IHM (cons_substitution y (tmVar (chi sigma (tmLam y M))) sigma) (fun z : ivar => if ivar_eq_dec (chi sigma (tmLam y M)) z then v else E z)).
+    apply eqnDom_sym in H.
+    apply eqnDom_sym, (eqnDom_trans _ _ _ H), eval_tm_ext.
+    intros z H0.
+    unfold cons_substitution.
+    destruct (ivar_eq_dec y z).
+    + unfold eval_tm.
+      destruct (ivar_eq_dec (chi sigma (tmLam y M)) (chi sigma (tmLam y M)))...
+    + apply eval_tm_ext.
+      intros z' H1.
+      destruct (ivar_eq_dec (chi sigma (tmLam y M)) z')...
+      subst.
+      assert (H2 : isFreshIn_substitution (chi sigma (tmLam y M)) sigma (tmLam y M) = true) by now apply main_property_of_chi.
+      unfold isFreshIn_substitution in H2.
+      rewrite forallb_true_iff in H2.
+      enough (H3 : isFreeIn (chi sigma (tmLam y M)) (sigma z) = false) by now rewrite H3 in H1.
+      apply negb_true_iff, H2, getFVs_isFreeIn.
+      simpl.
+      rewrite andb_true_iff, negb_true_iff, Nat.eqb_neq...
+Qed.
+
+End PreLambdaStructure.
+
+Class isLambdaStructure (Dom : Set) `{requiresPreLambdaStructure : isPreLambdaStructure Dom} : Type :=
+  { respect_beta : forall vv : Dom -> Dom, forall v0 : Dom, runApp (runLam vv) v0 =-= vv v0
+  ; respect_eta : forall v : Dom, runLam (runApp v) =-= v
+  }
+.
+
+#[global] Hint Resolve respect_beta : semantics_of_ulc.
+
+#[global] Hint Resolve respect_eta : semantics_of_ulc.
+
+End UntypedLamdbdaCalculus.
